Optimized compile function computes footprint in one pass
Signed-off-by: Craig Disselkoen <cdiss@amazon.com>

cedar-lean/Cedar/Thm/SymbolicCompilation.lean
@@ -220,4 +220,409 @@ theorem compile_well_typed {tx : TypedExpr} {Γ : TypeEnv} :
   exists t
   simp [hok, hwf_t, hty]
 
+def IsOption (tty : TermType) := ∃ tty', tty = TermType.option tty'
+def OptionTyped (t : Term) := IsOption t.typeOf
+
+/--
+Lemma
+-/
+private theorem typeOf_noneOf (tty : TermType) :
+  OptionTyped (Factory.noneOf tty)
+:= by
+  simp [OptionTyped, IsOption, Factory.noneOf, Term.typeOf]
+
+/--
+Lemma
+-/
+private theorem typeOf_someOf (t : Term) :
+  OptionTyped (⊙t)
+:= by
+  simp [OptionTyped, IsOption, Factory.someOf, Term.typeOf]
+
+/--
+Lemma
+-/
+private theorem typeOf_ite.simplify {c t f : Term} :
+  OptionTyped t → OptionTyped f → OptionTyped (Factory.ite.simplify c t f)
+:= by
+  simp only [OptionTyped, IsOption, Factory.ite.simplify, Bool.or_eq_true, decide_eq_true_eq,
+    forall_exists_index]
+  intro tty ht fty hf
+  split <;> rename_i h
+  · exists tty
+  · split
+    · exists fty
+    · split
+      · simp [Term.typeOf, TermPrim.typeOf] at ht
+      · simp [Term.typeOf, TermPrim.typeOf] at ht
+      · simp [Term.typeOf, TermPrim.typeOf] at hf
+      · simp [Term.typeOf, TermPrim.typeOf] at ht
+      · simp [Term.typeOf] ; exists tty
+
+/--
+Lemma
+-/
+private theorem typeOf_ite {c t f : Term} :
+  OptionTyped t → OptionTyped f → OptionTyped (Factory.ite c t f)
+:= by
+  intro ht hf
+  simp only [OptionTyped, IsOption, Factory.ite]
+  split
+  · simp [Term.typeOf]
+  · apply typeOf_ite.simplify ht hf
+
+/--
+Lemma
+-/
+private theorem typeOf_ifFalse {g t : Term} :
+  OptionTyped (Factory.ifFalse g t)
+:= by
+  simp only [Factory.ifFalse]
+  apply typeOf_ite
+  · apply typeOf_noneOf
+  · apply typeOf_someOf
+
+/--
+Lemma
+-/
+private theorem typeOf_ifTrue {g t : Term} :
+  OptionTyped (Factory.ifTrue g t)
+:= by
+  simp only [Factory.ifTrue]
+  apply typeOf_ite
+  · apply typeOf_someOf
+  · apply typeOf_noneOf
+
+/--
+Lemma
+-/
+private theorem typeOf_ifSome {g t : Term} :
+  OptionTyped t → OptionTyped (Factory.ifSome g t)
+:= by
+  intro ht
+  simp only [OptionTyped, IsOption, Factory.ifSome]
+  split
+  · apply typeOf_ite _ ht
+    apply typeOf_noneOf
+  · apply typeOf_ifFalse
+
+/--
+Lemma
+-/
+private theorem typeOf_ifAllSome {gs : List Term} {t : Term} :
+  OptionTyped t → OptionTyped (Factory.ifAllSome gs t)
+:= by
+  simp only [Factory.ifAllSome]
+  split
+  · apply typeOf_ite
+    apply typeOf_noneOf
+  · intro h ; apply typeOf_ifFalse
+
+/--
+Weaker result than `compile_well_typed`, but requiring weaker hypotheses:
+
+If `compile` on any expression (not necessarily well-typed) produces `.ok t`,
+then `t` must have option type
+-/
+theorem compile_ok_implies_option {x : Expr} {εnv : SymEnv} {t : Term} :
+  compile x εnv = .ok t →
+  ∃ tty, t.typeOf = .option tty
+:= by
+  cases x <;> simp [compile]
+  case lit p =>
+    cases p <;> simp [compilePrim]
+    case bool | int | string =>
+      intro h ; subst t
+      apply typeOf_someOf
+    case entityUID =>
+      split <;> simp
+      intro h ; subst t
+      apply typeOf_someOf
+  case var v =>
+    cases v <;> simp [compileVar]
+    all_goals {
+      split <;> simp only [Except.ok.injEq, reduceCtorEq, false_implies]
+      intro h ; subst t
+      apply typeOf_someOf
+    }
+  case and x₁ x₂ | or x₁ x₂ =>
+    cases hx₁ : compile x₁ εnv <;> simp [compileAnd, compileOr]
+    case ok t₁ =>
+      replace ⟨tty₁, hx₁⟩ := compile_ok_implies_option hx₁
+      split <;> simp [Term.typeOf] at *
+      · subst tty₁ ; intro h ; subst t ; simp [Term.typeOf]
+      · cases hx₂ : compile x₂ εnv <;> simp
+        case ok t₂ =>
+          replace ⟨tty₂, hx₂⟩ := compile_ok_implies_option hx₂
+          split <;> simp only [Except.ok.injEq, reduceCtorEq, false_implies]
+          · intro h ; subst t
+            apply typeOf_ifSome
+            apply typeOf_ite
+            repeat first
+            | { simp [OptionTyped, IsOption, hx₂] }
+            | { apply typeOf_someOf }
+  case ite x₁ x₂ x₃ =>
+    cases hx₁ : compile x₁ εnv <;> simp [compileIf]
+    case ok t₁ =>
+      replace ⟨tty₁, hx₁⟩ := compile_ok_implies_option hx₁
+      split <;> simp [Term.typeOf] at *
+      · subst tty₁
+        intro hx₂ ; simp [compile_ok_implies_option hx₂]
+      · subst tty₁
+        intro hx₃ ; simp [compile_ok_implies_option hx₃]
+      · cases hx₂ : compile x₂ εnv <;> simp
+        case ok t₂ =>
+          replace ⟨tty₂, hx₂⟩ := compile_ok_implies_option hx₂
+          cases hx₃ : compile x₃ εnv <;> simp
+          case ok t₃ =>
+            replace ⟨tty₃, hx₃⟩ := compile_ok_implies_option hx₃
+            split <;> simp only [Except.ok.injEq, reduceCtorEq, false_implies]
+            · intro h ; subst h
+              apply typeOf_ifSome
+              apply typeOf_ite
+              all_goals simp [OptionTyped, IsOption, *]
+  case unaryApp op x =>
+    cases hx : compile x εnv <;> simp [compileApp₁]
+    case ok t =>
+      replace ⟨tty, hx⟩ := compile_ok_implies_option hx
+      split <;> simp only [Except.bind_ok, Except.ok.injEq, Except.bind_err, reduceCtorEq, false_implies]
+      <;> intro h <;> subst h <;> rename_i h
+      <;> apply typeOf_ifSome
+      · apply typeOf_someOf
+      · apply typeOf_ifFalse
+      · apply typeOf_someOf
+      · apply typeOf_someOf
+      · apply typeOf_someOf
+  case binaryApp op x₁ x₂ =>
+    cases hx₁ : compile x₁ εnv <;> simp [compileApp₂]
+    case ok t₁ =>
+      replace ⟨tty₁, hx₁⟩ := compile_ok_implies_option hx₁
+      cases hx₂ : compile x₂ εnv <;> simp only [Except.bind_ok, Except.bind_err, reduceCtorEq, false_implies]
+      case ok t₂ =>
+        replace ⟨tty₂, hx₂⟩ := compile_ok_implies_option hx₂
+        split
+        case _ =>
+          cases reducibleEq (Factory.option.get t₁).typeOf (Factory.option.get t₂).typeOf <;> simp
+          case ok b =>
+          split <;> simp only [Except.bind_ok, Except.ok.injEq]
+          <;> intro h <;> subst t <;> apply typeOf_ifSome
+          <;> simp only [OptionTyped, IsOption]
+          <;> apply typeOf_ifSome
+          <;> apply typeOf_someOf
+        case _ | _ | _ | _ | _ | _ =>
+          simp only [Except.bind_ok, Except.ok.injEq]
+          intro h ; subst t
+          apply typeOf_ifSome
+          apply typeOf_ifSome
+          apply typeOf_someOf
+        case _ | _ | _ =>
+          simp only [Except.bind_ok, Except.ok.injEq]
+          intro h ; subst t
+          apply typeOf_ifSome
+          apply typeOf_ifSome
+          apply typeOf_ifFalse
+        case _ =>
+          cases (Factory.option.get t₂).typeOf
+          case prim | option | set | record =>
+            split <;> simp only [Except.bind_ok, Except.ok.injEq, Except.bind_err, reduceCtorEq, false_implies]
+            intro h ; subst t
+            apply typeOf_ifSome
+            apply typeOf_ifSome
+            apply typeOf_someOf
+        case _ | _ =>
+          split <;> simp only [Except.bind_ok, Except.ok.injEq, Except.bind_err, reduceCtorEq, false_implies]
+          intro h ; subst t
+          apply typeOf_ifSome
+          apply typeOf_ifSome
+          apply typeOf_someOf
+        case _ | _ =>
+          simp only [Except.bind_ok, Except.ok.injEq]
+          intro h ; subst t
+          apply typeOf_ifSome
+          apply typeOf_ifSome
+          apply typeOf_someOf
+        case _ =>
+          rename_i ety _ _
+          cases htag : compileHasTag (Factory.option.get t₁) (Factory.option.get t₂) (εnv.entities.tags ety)
+          <;> simp only [Except.bind_ok, Except.ok.injEq, Except.bind_err, reduceCtorEq, false_implies]
+          case ok t' =>
+          intro h ; subst t
+          apply typeOf_ifSome
+          apply typeOf_ifSome
+          simp only [compileHasTag] at htag
+          split at htag <;> simp only [Except.ok.injEq, reduceCtorEq] at htag
+          <;> subst htag
+          <;> apply typeOf_someOf
+        case _ =>
+          rename_i ety _ _
+          cases htag : compileGetTag (Factory.option.get t₁) (Factory.option.get t₂) (εnv.entities.tags ety)
+          <;> simp only [Except.bind_ok, Except.ok.injEq, Except.bind_err, reduceCtorEq, false_implies]
+          case ok t' =>
+          intro h ; subst t
+          apply typeOf_ifSome
+          apply typeOf_ifSome
+          simp only [compileGetTag] at htag
+          split at htag <;> simp only [Except.ok.injEq, reduceCtorEq] at htag
+          subst htag
+          simp only [SymTags.getTag]
+          apply typeOf_ifTrue
+        case _ => simp
+  case hasAttr x attr =>
+    cases hx : compile x εnv <;> simp only [Except.bind_ok, Except.bind_err, reduceCtorEq, false_implies]
+    case ok t' =>
+    replace ⟨tty, hx⟩ := compile_ok_implies_option hx
+    cases hattr : compileHasAttr (Factory.option.get t') attr εnv.entities
+    <;> simp only [Except.bind_ok, Except.ok.injEq, Except.bind_err, reduceCtorEq, false_implies]
+    case ok t'' =>
+    intro h ; subst t
+    apply typeOf_ifSome
+    simp only [compileHasAttr] at hattr
+    cases hattrs : compileAttrsOf (Factory.option.get t') εnv.entities
+    <;> simp only [hattrs, Except.bind_ok, Except.bind_err, reduceCtorEq] at hattr
+    split at hattr
+    · split at hattr <;> simp only [Except.ok.injEq] at hattr
+      <;> subst hattr
+      <;> apply typeOf_someOf
+    · simp at hattr
+  case getAttr x attr =>
+    cases hx : compile x εnv <;> simp only [Except.bind_ok, Except.bind_err, reduceCtorEq, false_implies]
+    case ok t' =>
+    replace ⟨tty, hx⟩ := compile_ok_implies_option hx
+    cases hattr : compileGetAttr (Factory.option.get t') attr εnv.entities
+    <;> simp only [Except.bind_ok, Except.ok.injEq, Except.bind_err, reduceCtorEq, false_implies]
+    case ok t'' =>
+    intro h ; subst t
+    apply typeOf_ifSome
+    simp only [compileGetAttr] at hattr
+    cases hattrs : compileAttrsOf (Factory.option.get t') εnv.entities
+    <;> simp only [hattrs, Except.bind_ok, Except.bind_err, reduceCtorEq] at hattr
+    split at hattr <;> rename_i h₁
+    · split at hattr <;> simp only [Except.ok.injEq, reduceCtorEq] at hattr
+      <;> subst hattr
+      · rename_i attrTy hattrTy
+        exists attrTy
+        simp only [Factory.record.get]
+        split
+        · split <;> rename_i h₂
+          · have h₃ := typeOf_term_record_attr_value_typeOf h₁ h₂
+            simp [hattrTy] at h₃ ; simp [← h₃]
+          · exfalso
+            have ⟨t'', h₃⟩ := typeOf_term_record_attr_value h₁ hattrTy
+            apply h₂ t'' h₃.left
+        · split <;> rename_i h₂
+          · split
+            · simp only [Term.typeOf]
+              simp only [compileAttrsOf] at hattrs
+              split at hattrs
+              · split at hattrs <;> simp only [Except.ok.injEq, reduceCtorEq] at hattrs
+                subst hattrs
+                simp [h₁] at h₂ ; subst h₂
+                rename_i h₂
+                simp [hattrTy] at h₂ ; simp [h₂]
+              · simp only [Except.ok.injEq] at hattrs ; subst hattrs
+                rename_i h _ ; simp [h₁] at h ; subst h
+                simp [h₁] at h₂ ; subst h₂
+                rename_i h₂
+                simp [hattrTy] at h₂ ; simp [h₂]
+              · simp at hattrs
+            · exfalso
+              simp [h₁] at h₂ ; subst h₂
+              rename_i h₂ ; apply h₂ attrTy.option hattrTy
+          · exfalso
+            apply h₂ _ h₁
+      · apply typeOf_someOf
+    · simp at hattr
+  case set xs =>
+    cases hxs : xs.mapM₁ λ x => compile x.val εnv
+    <;> rw [List.mapM₁_eq_mapM (compile · εnv)] at hxs
+    <;> simp only [Except.bind_ok, Except.bind_err, reduceCtorEq, false_implies]
+    simp only [compileSet, List.all_eq_true, decide_eq_true_eq]
+    split <;> simp only [reduceCtorEq, false_implies, List.mem_cons, forall_eq_or_imp, List.map_cons]
+    split <;> simp only [*, true_and, reduceCtorEq, false_implies]
+    split <;> simp only [Except.ok.injEq, reduceCtorEq, false_implies]
+    intro h ; subst t
+    apply typeOf_ifAllSome
+    apply typeOf_someOf
+  case call xfn xs =>
+    cases hxs : xs.mapM₁ λ x => compile x.val εnv
+    <;> rw [List.mapM₁_eq_mapM (compile · εnv)] at hxs
+    <;> simp only [Except.bind_ok, Except.bind_err, reduceCtorEq, false_implies]
+    simp only [compileCall]
+    split
+    case _ =>
+      simp only [compileCall₀]
+      split
+      · split <;> simp only [Except.ok.injEq, reduceCtorEq, false_implies]
+        intro h ; subst t
+        apply typeOf_someOf
+      · simp only [reduceCtorEq, false_implies]
+    case _ | _ | _ | _ =>
+      simp only [compileCall₂, compileCallWithError₂]
+      split <;> simp only [Except.ok.injEq, reduceCtorEq, false_implies]
+      intro h ; subst t
+      apply typeOf_ifSome
+      apply typeOf_ifSome
+      apply typeOf_someOf
+    case _ =>
+      simp only [compileCall₀]
+      split
+      · split <;> simp only [Except.ok.injEq, reduceCtorEq, false_implies]
+        intro h ; subst t
+        apply typeOf_someOf
+      · simp only [reduceCtorEq, false_implies]
+    case _ | _ | _ | _ =>
+      simp only [compileCall₁, compileCallWithError₁]
+      split <;> simp only [Except.ok.injEq, reduceCtorEq, false_implies]
+      intro h ; subst t
+      apply typeOf_ifSome
+      apply typeOf_someOf
+    case _ =>
+      simp only [compileCall₂, compileCallWithError₂]
+      split <;> simp only [Except.ok.injEq, reduceCtorEq, false_implies]
+      intro h ; subst t
+      apply typeOf_ifSome
+      apply typeOf_ifSome
+      apply typeOf_someOf
+    case _ | _ =>
+      simp only [compileCall₀]
+      split
+      · split <;> simp only [Except.ok.injEq, reduceCtorEq, false_implies]
+        intro h ; subst t
+        apply typeOf_someOf
+      · simp only [reduceCtorEq, false_implies]
+    case _ | _ =>
+      simp only [compileCallWithError₂, Bool.and_eq_true, decide_eq_true_eq]
+      split <;> simp only [Except.ok.injEq, reduceCtorEq, false_implies]
+      intro h ; subst t
+      apply typeOf_ifSome
+      apply typeOf_ifSome
+      simp only [Datetime.offset, Datetime.durationSince]
+      apply typeOf_ifFalse
+    case _ =>
+      simp only [compileCallWithError₁]
+      split <;> simp only [Except.ok.injEq, reduceCtorEq, false_implies]
+      intro h ; subst t
+      apply typeOf_ifSome
+      simp only [Datetime.toDate]
+      apply typeOf_ite
+      · apply typeOf_someOf
+      · apply typeOf_ite
+        · apply typeOf_someOf
+        · apply typeOf_ifFalse
+    case _ | _ | _ | _ | _ | _ =>
+      simp only [compileCall₁, compileCallWithError₁]
+      split <;> simp only [Except.ok.injEq, reduceCtorEq, false_implies]
+      intro h ; subst t
+      apply typeOf_ifSome
+      apply typeOf_someOf
+    case _ => simp
+  case record m =>
+    simp [do_eq_ok] ; intro m' hm h ; subst t
+    simp_do_let (m.mapM₂ (λ ⟨(a₁, x₁), _⟩ => do .ok (a₁, ← compile x₁ εnv))) at hm
+    simp only [Except.ok.injEq] at hm ; subst hm
+    rename_i m' hm
+    simp only [compileRecord]
+    apply typeOf_ifAllSome
+    apply typeOf_someOf
+
 end Cedar.Thm
