cedar-lean/Cedar/SymCCOpt/Authorizer.lean
@@ -1,0 +1,43 @@
+/-
+ Copyright Cedar Contributors
+
+ Licensed under the Apache License, Version 2.0 (the "License");
+ you may not use this file except in compliance with the License.
+ You may obtain a copy of the License at
+
+      https://www.apache.org/licenses/LICENSE-2.0
+
+ Unless required by applicable law or agreed to in writing, software
+ distributed under the License is distributed on an "AS IS" BASIS,
+ WITHOUT WARRANTIES OR CONDITIONS OF ANY KIND, either express or implied.
+ See the License for the specific language governing permissions and
+ limitations under the License.
+-/
+
+import Cedar.SymCCOpt.Compiler
+
+namespace Cedar.SymCC.Opt
+
+open Factory Cedar.Spec
+
+def compileWithEffect (effect : Effect) (policy : Policy) (εnv : SymEnv) : Result (Option CompileResult) :=
+  if policy.effect == effect
+  then Opt.compile policy.toExpr εnv
+  else .ok .none
+
+def satisfiedPolicies (effect : Effect) (policies : Policies) (εnv : SymEnv) : Result CompileResult := do
+  let ress ← policies.filterMapM (compileWithEffect effect · εnv)
+  .ok {
+    term := anyTrue (eq · (someOf true)) (ress.map CompileResult.term)
+    footprint := ress.mapUnion CompileResult.footprint
+  }
+
+def isAuthorized (policies : Policies) (εnv : SymEnv) : Result CompileResult := do
+  let forbids ← satisfiedPolicies .forbid policies εnv
+  let permits ← satisfiedPolicies .permit policies εnv
+  .ok {
+    term := and permits.term (not forbids.term)
+    footprint := permits.footprint ∪ forbids.footprint
+  }
+
+end Cedar.SymCC.Opt
