cedar-lean/Cedar/SymCCOpt/Compiler.lean
@@ -1,0 +1,399 @@
+/-
+ Copyright Cedar Contributors
+
+ Licensed under the Apache License, Version 2.0 (the "License");
+ you may not use this file except in compliance with the License.
+ You may obtain a copy of the License at
+
+      https://www.apache.org/licenses/LICENSE-2.0
+
+ Unless required by applicable law or agreed to in writing, software
+ distributed under the License is distributed on an "AS IS" BASIS,
+ WITHOUT WARRANTIES OR CONDITIONS OF ANY KIND, either express or implied.
+ See the License for the specific language governing permissions and
+ limitations under the License.
+-/
+
+import Cedar.SymCC.Compiler
+import Cedar.SymCC.Env
+import Cedar.SymCC.ExtFun
+import Cedar.SymCC.Factory
+
+/-!
+This file defines an optimized Cedar symbolic compiler, which computes the
+actual compiled `Term` and the `footprint` simultaneously, avoiding the
+inefficiencies in the `footprint` function in SymCC/Enforcer.lean, which
+repeatedly calls `compile` on certain subexpressions, making it quadratic or
+worse in policy size, at least for certain policies.
+
+For notes on the meaning of compile or footprint, see SymCC/Compiler.lean and
+SymCC/Enforcer.lean, which have clearer, unoptimized implementations.
+-/
+
+namespace Cedar.SymCC.Opt
+
+open Cedar.Data Cedar.Spec Cedar.Validation
+open Factory
+
+/--
+Structure returned by the optimized compiler, as opposed to the unoptimized
+compiler which just produces a `Term`
+-/
+structure CompileResult where
+  /-- Well-formed term of the appropriate type, representing the compiled expression -/
+  term : Term
+  /--
+  The "footprint" of the compiled expression.
+
+  This is the terms corresponding to subexpressions of the compiled expression
+  of the following form:
+
+  * A variable term with an entity type
+  * An entity reference literal
+  * An attribute access expression with an entity type
+  * A binary (`getTag`) expression with an entity type
+
+  These are the only basic expressions in Cedar that may evaluate to an entity.
+  All other expressions that evaluate to an entity are built up from the above
+  basic expresions.
+
+  All terms in the `footprint` are of type `TermType.option .entity`.
+  -/
+  footprint : Set Term
+
+/-- Map on the `Term`, leaving the `footprint` unchanged -/
+def CompileResult.mapTerm (f : Term → Term) : CompileResult → CompileResult
+  | { term, footprint } => { term := f term, footprint }
+
+/--
+Return the footprint of this compiled term _itself_ (not counting its subexpressions).
+Only terms of option-entity type have any direct footprint.
+
+This corresponds to `ofEntity` in the `footprint` function in
+SymCC/Enforcer.lean, except that we only call it when compiling to `Term` was
+successful, so it takes a `Term` argument rather than `Result Term`.
+-/
+def directFootprint (t : Term) : Set Term :=
+  if t.typeOf.isOptionEntityType then Set.singleton t else Set.empty
+
+def compilePrim (p : Prim) (εs : SymEntities) : Result CompileResult :=
+  match p with
+  | .bool b        => .ok { term := ⊙b, footprint := ∅ }
+  | .int i         => .ok { term := ⊙i, footprint := ∅ }
+  | .string s      => .ok { term := ⊙s, footprint := ∅ }
+  | .entityUID uid =>
+      if εs.isValidEntityUID uid then
+        -- essentially inlining our `directFootprint` function, no need to
+        -- compute `.typeOf`, we know the term is option-entity type
+        let term := ⊙uid
+        .ok { term, footprint := Set.singleton term }
+      else
+        .error .typeError
+
+def compileVar (v : Var) (req : SymRequest) : Result CompileResult :=
+  match v with
+  | .principal =>
+      if req.principal.typeOf.isEntityType then
+        -- essentially inlining our `directFootprint` function, no need to
+        -- compute `.typeOf`, we know the term is option-entity type
+        let term := ⊙req.principal
+        .ok { term, footprint := Set.singleton term }
+      else
+        .error .typeError
+  | .action    =>
+      if req.action.typeOf.isEntityType then
+        -- essentially inlining our `directFootprint` function, no need to
+        -- compute `.typeOf`, we know the term is option-entity type
+        let term := ⊙req.action
+        .ok { term, footprint := Set.singleton term }
+      else
+        .error .typeError
+  | .resource  =>
+      if req.resource.typeOf.isEntityType then
+        -- essentially inlining our `directFootprint` function, no need to
+        -- compute `.typeOf`, we know the term is option-entity type
+        let term := ⊙req.resource
+        .ok { term, footprint := Set.singleton term }
+      else
+        .error .typeError
+  | .context   =>
+      if req.context.typeOf.isRecordType then
+        -- essentially inlining our `directFootprint` function, no need to
+        -- compute `.typeOf`, we know the term is _not_ option-entity type
+        .ok { term := ⊙req.context, footprint := ∅ }
+      else
+        .error .typeError
+
+def compileApp₁ (op₁ : UnaryOp) (arg : CompileResult) : Result CompileResult := do
+  match op₁, arg.term.typeOf with
+  | .not, .bool            => arg.mapTerm λ term => ⊙not term
+  | .neg, .bitvec 64       => arg.mapTerm λ term => ifFalse (bvnego term) (bvneg term)
+  | .like p, .string       => arg.mapTerm λ term => ⊙string.like term p
+  | .is ety₁, .entity ety₂ => arg.mapTerm λ _ => ⊙(ety₁ = ety₂ : Bool)
+  | .isEmpty, .set _       => arg.mapTerm λ term => ⊙set.isEmpty term
+  | _, _                   => .error .typeError
+
+def compileApp₂ (op₂ : BinaryOp) (arg₁ arg₂ : CompileResult) (εs : SymEntities) : Result CompileResult := do
+  -- compute the footprint of the arguments, not counting the contribution of the `directFootprint` of
+  -- the binaryOp term (if any) (particularly relevant for `getTag`)
+  let argsFootprint := arg₁.footprint ∪ arg₂.footprint
+  -- mimicking the behavior of the unoptimized compiler in how the direct
+  -- footprint for the binaryOp term itself is computed
+  let binaryOpFootprint := λ term => directFootprint (ifSome arg₁.term (ifSome arg₂.term term))
+  -- for the rest of this function, we consider only the `option.get`-ed args.
+  -- see detailed note in the toplevel optimized `compile` function below.
+  let t₁ := option.get arg₁.term
+  let t₂ := option.get arg₂.term
+  match op₂, t₁.typeOf, t₂.typeOf with
+  | .eq, ty₁, ty₂                           => let term := if (← reducibleEq ty₁ ty₂) then ⊙eq t₁ t₂ else ⊙false
+                                               .ok { term, footprint := argsFootprint ∪ binaryOpFootprint term } -- assuming everything is well-typed, the `binaryOpFootprint` term here will be ∅, but: (1) we want the two compilers to agree even on non-well-typed inputs, for ease of proofs; and (2) the unoptimized compiler adds this term
+  | .less, .bitvec 64, .bitvec 64           => let term := ⊙bvslt t₁ t₂
+                                               .ok { term, footprint := argsFootprint ∪ binaryOpFootprint term } -- assuming everything is well-typed, the `binaryOpFootprint` term here will be ∅, but: (1) we want the two compilers to agree even on non-well-typed inputs, for ease of proofs; and (2) the unoptimized compiler adds this term
+  | .less, .ext .datetime, .ext .datetime   => let term := ⊙bvslt (ext.datetime.val t₁) (ext.datetime.val t₂)
+                                               .ok { term, footprint := argsFootprint ∪ binaryOpFootprint term } -- assuming everything is well-typed, the `binaryOpFootprint` term here will be ∅, but: (1) we want the two compilers to agree even on non-well-typed inputs, for ease of proofs; and (2) the unoptimized compiler adds this term
+  | .less, .ext .duration, .ext .duration   => let term := ⊙bvslt (ext.duration.val t₁) (ext.duration.val t₂)
+                                               .ok { term, footprint := argsFootprint ∪ binaryOpFootprint term } -- assuming everything is well-typed, the `binaryOpFootprint` term here will be ∅, but: (1) we want the two compilers to agree even on non-well-typed inputs, for ease of proofs; and (2) the unoptimized compiler adds this term
+  | .lessEq, .bitvec 64, .bitvec 64         => let term := ⊙bvsle t₁ t₂
+                                               .ok { term, footprint := argsFootprint ∪ binaryOpFootprint term } -- assuming everything is well-typed, the `binaryOpFootprint` term here will be ∅, but: (1) we want the two compilers to agree even on non-well-typed inputs, for ease of proofs; and (2) the unoptimized compiler adds this term
+  | .lessEq, .ext .datetime, .ext .datetime => let term := ⊙bvsle (ext.datetime.val t₁) (ext.datetime.val t₂)
+                                               .ok { term, footprint := argsFootprint ∪ binaryOpFootprint term } -- assuming everything is well-typed, the `binaryOpFootprint` term here will be ∅, but: (1) we want the two compilers to agree even on non-well-typed inputs, for ease of proofs; and (2) the unoptimized compiler adds this term
+  | .lessEq, .ext .duration, .ext .duration => let term := ⊙bvsle (ext.duration.val t₁) (ext.duration.val t₂)
+                                               .ok { term, footprint := argsFootprint ∪ binaryOpFootprint term } -- assuming everything is well-typed, the `binaryOpFootprint` term here will be ∅, but: (1) we want the two compilers to agree even on non-well-typed inputs, for ease of proofs; and (2) the unoptimized compiler adds this term
+  | .add, .bitvec 64, .bitvec 64            => let term := ifFalse (bvsaddo t₁ t₂) (bvadd t₁ t₂)
+                                               .ok { term, footprint := argsFootprint ∪ binaryOpFootprint term } -- assuming everything is well-typed, the `binaryOpFootprint` term here will be ∅, but: (1) we want the two compilers to agree even on non-well-typed inputs, for ease of proofs; and (2) the unoptimized compiler adds this term
+  | .sub, .bitvec 64, .bitvec 64            => let term := ifFalse (bvssubo t₁ t₂) (bvsub t₁ t₂)
+                                               .ok { term, footprint := argsFootprint ∪ binaryOpFootprint term } -- assuming everything is well-typed, the `binaryOpFootprint` term here will be ∅, but: (1) we want the two compilers to agree even on non-well-typed inputs, for ease of proofs; and (2) the unoptimized compiler adds this term
+  | .mul, .bitvec 64, .bitvec 64            => let term := ifFalse (bvsmulo t₁ t₂) (bvmul t₁ t₂)
+                                               .ok { term, footprint := argsFootprint ∪ binaryOpFootprint term } -- assuming everything is well-typed, the `binaryOpFootprint` term here will be ∅, but: (1) we want the two compilers to agree even on non-well-typed inputs, for ease of proofs; and (2) the unoptimized compiler adds this term
+  | .contains, .set ty₁, ty₂                => if ty₁ = ty₂
+                                                then
+                                                  let term := ⊙set.member t₂ t₁
+                                                  .ok { term, footprint := argsFootprint ∪ binaryOpFootprint term } -- assuming everything is well-typed, the `binaryOpFootprint` term here will be ∅, but: (1) we want the two compilers to agree even on non-well-typed inputs, for ease of proofs; and (2) the unoptimized compiler adds this term
+                                                else .error .typeError
+  | .containsAll, .set ty₁, .set ty₂        => if ty₁ = ty₂
+                                                then
+                                                  let term := ⊙set.subset t₂ t₁
+                                                  .ok { term, footprint := argsFootprint ∪ binaryOpFootprint term } -- assuming everything is well-typed, the `binaryOpFootprint` term here will be ∅, but: (1) we want the two compilers to agree even on non-well-typed inputs, for ease of proofs; and (2) the unoptimized compiler adds this term
+                                                else .error .typeError
+  | .containsAny, .set ty₁, .set ty₂        => if ty₁ = ty₂
+                                                then
+                                                  let term := ⊙set.intersects t₁ t₂
+                                                  .ok { term, footprint := argsFootprint ∪ binaryOpFootprint term } -- assuming everything is well-typed, the `binaryOpFootprint` term here will be ∅, but: (1) we want the two compilers to agree even on non-well-typed inputs, for ease of proofs; and (2) the unoptimized compiler adds this term
+                                                else .error .typeError
+  | .mem, .entity ety₁, .entity ety₂        => let term := ⊙compileInₑ t₁ t₂ (εs.ancestorsOfType ety₁ ety₂)
+                                               .ok { term, footprint := argsFootprint ∪ binaryOpFootprint term } -- assuming everything is well-typed, the `binaryOpFootprint` term here will be ∅, but: (1) we want the two compilers to agree even on non-well-typed inputs, for ease of proofs; and (2) the unoptimized compiler adds this term
+  | .mem, .entity ety₁, .set (.entity ety₂) => let term := ⊙compileInₛ t₁ t₂ (εs.ancestorsOfType ety₁ ety₂)
+                                               .ok { term, footprint := argsFootprint ∪ binaryOpFootprint term } -- assuming everything is well-typed, the `binaryOpFootprint` term here will be ∅, but: (1) we want the two compilers to agree even on non-well-typed inputs, for ease of proofs; and (2) the unoptimized compiler adds this term
+  | .hasTag, .entity ety, .string           => let term ← compileHasTag t₁ t₂ (εs.tags ety)
+                                               .ok { term, footprint := argsFootprint ∪ binaryOpFootprint term } -- assuming everything is well-typed, the `binaryOpFootprint` term here will be ∅, but: (1) we want the two compilers to agree even on non-well-typed inputs, for ease of proofs; and (2) the unoptimized compiler adds this term
+  | .getTag, .entity ety, .string           => let term ← compileGetTag t₁ t₂ (εs.tags ety)
+                                               .ok { term, footprint := argsFootprint ∪ binaryOpFootprint term } -- in this `getTag` case, the `binaryOpFootprint` term could actually be nonempty, in the case where the tags are entity-typed
+  | _, _, _                                 => .error .typeError
+
+def compileHasAttr (arg : CompileResult) (a : Attr) (εs : SymEntities) : Result CompileResult := do
+  let attrs ← compileAttrsOf arg.term εs
+  match attrs.typeOf with
+  | .record rty =>
+    match rty.find? a with
+    | .some (.option _) => .ok { term := ⊙isSome (record.get attrs a), footprint := arg.footprint }
+    | .some _           => .ok { term := ⊙true, footprint := arg.footprint }
+    | .none             => .ok { term := ⊙false, footprint := arg.footprint }
+  | _ => .error .typeError
+
+def compileGetAttr (arg : CompileResult) (a : Attr) (εs : SymEntities) : Result CompileResult := do
+  -- mimicking the behavior of the unoptimized compiler in how the direct
+  -- footprint for the getAttr term itself is computed
+  let getAttrFootprint := λ term => directFootprint (ifSome arg.term term)
+  -- for the rest of this function, we consider only the `option.get`-ed args.
+  -- see detailed note in the toplevel optimized `compile` function below.
+  let term := option.get arg.term
+  let attrs ← compileAttrsOf term εs
+  match attrs.typeOf with
+  | .record rty =>
+    let term ← match rty.find? a with
+    | .some (.option _) => record.get attrs a
+    | .some _           => ⊙(record.get attrs a)
+    | .none             => .error .noSuchAttribute
+    .ok { term, footprint := getAttrFootprint term ∪ arg.footprint }
+  | _ => .error .typeError
+
+def compileIf (arg₁ : CompileResult) (arg₂ arg₃ : Result CompileResult) : Result CompileResult := do
+  match arg₁.term, arg₁.term.typeOf with
+  | .some (.prim (.bool true)), _  => arg₂ -- omitting arg₁.footprint is sound: unoptimized `SymCC.footprint` does that in this case, and our proofs show it's sound
+  | .some (.prim (.bool false)), _ => arg₃ -- omitting arg₁.footprint is sound: unoptimized `SymCC.footprint` does that in this case, and our proofs show it's sound
+  | _, .option .bool =>
+    let arg₂ ← arg₂
+    let arg₃ ← arg₃
+    if arg₂.term.typeOf = arg₃.term.typeOf
+    then .ok {
+      term := ifSome arg₁.term (ite (option.get arg₁.term) arg₂.term arg₃.term)
+      footprint := arg₁.footprint ∪ arg₂.footprint ∪ arg₃.footprint
+    }
+    else .error .typeError
+  | _, _ => .error .typeError
+
+def compileAnd (arg₁ : CompileResult) (arg₂ : Result CompileResult) : Result CompileResult := do
+  match arg₁.term, arg₁.term.typeOf with
+  | .some (.prim (.bool false)), _ => .ok { term := arg₁.term, footprint := ∅ } -- we could just do `.ok arg₁`, but the unoptimized `SymCC.footprint` returns an empty footprint in this case, which is also sound (as our proofs show)
+  | _, .option .bool =>
+    let arg₂ ← arg₂
+    if arg₂.term.typeOf = .option .bool
+    then
+      let footprint := if arg₁.term = .some (.prim (.bool true))
+        then arg₂.footprint -- omitting arg₁.footprint is sound: unoptimized `SymCC.footprint` does that in this case, and our proofs show it's sound
+        else arg₁.footprint ∪ arg₂.footprint
+      .ok {
+        term := ifSome arg₁.term (ite (option.get arg₁.term) arg₂.term (⊙false))
+        footprint
+      }
+    else .error .typeError
+  | _, _ => .error .typeError
+
+def compileOr (arg₁ : CompileResult) (arg₂ : Result CompileResult) : Result CompileResult := do
+  match arg₁.term, arg₁.term.typeOf with
+  | .some (.prim (.bool true)), _  => .ok { term := arg₁.term, footprint := ∅ } -- we could just do `.ok arg₁`, but the unoptimized `SymCC.footprint` returns an empty footprint in this case, which is also sound (as our proofs show)
+  | _, .option .bool =>
+    let arg₂ ← arg₂
+    if arg₂.term.typeOf = .option .bool
+    then
+      let footprint := if arg₁.term = .some (.prim (.bool false))
+        then arg₂.footprint -- omitting arg₁.footprint is sound: unoptimized `SymCC.footprint` does that in this case, and our proofs show it's sound
+        else arg₁.footprint ∪ arg₂.footprint
+      .ok {
+        term := ifSome arg₁.term (ite (option.get arg₁.term) (⊙true) arg₂.term)
+        footprint
+      }
+    else .error .typeError
+  | _, _ => .error .typeError
+
+def compileSet (args : List CompileResult) : Result CompileResult := do
+   match args with
+    | []     => .error .unsupportedError  -- reject empty set literals
+    | arg :: _ =>
+      match arg.term.typeOf with
+      | .option ty =>
+        let terms := args.map CompileResult.term
+        if terms.all (Term.typeOf · = .option ty)
+        then .ok {
+          term := ifAllSome terms (⊙setOf (terms.map option.get) ty)
+          footprint := args.mapUnion CompileResult.footprint
+        }
+        else .error .typeError
+      | _ => .error .typeError
+
+def compileRecord (ats : List (Attr × CompileResult)) : CompileResult :=
+  let terms := ats.map λ ⟨_, { term, .. }⟩ => term
+  {
+    term := ifAllSome terms (⊙recordOf (ats.map (Prod.map id (λ { term, .. } => option.get term))))
+    footprint := ats.mapUnion λ ⟨_, { footprint, .. }⟩ => footprint
+  }
+
+def compileCall₀ {α} [Coe α Ext] (mk : String → Option α) : CompileResult → Result CompileResult
+  | { term := .some (.prim (.string s)), footprint } =>
+    match (mk s) with
+    | .some v => .ok { term := ⊙ .prim (.ext v), footprint }
+    | .none   => .error .typeError
+  | _         => .error .typeError
+
+def compileCallWithError₁ (xty : ExtType) (enc : Term -> Term) (arg₁ : CompileResult) : Result CompileResult := do
+  if arg₁.term.typeOf = .option (.ext xty)
+  then .ok {
+    term := ifSome arg₁.term (enc (option.get arg₁.term))
+    footprint := arg₁.footprint
+  }
+  else .error .typeError
+
+def compileCall₁ (xty : ExtType) (enc : Term → Term) (arg₁ : CompileResult) : Result CompileResult :=
+  compileCallWithError₁ xty (λ t₁ => ⊙ enc t₁) arg₁
+
+def compileCallWithError₂ (xty₁ xty₂ : ExtType) (enc : Term → Term → Term) (arg₁ arg₂ : CompileResult) : Result CompileResult := do
+  let ty₁ := .option (.ext xty₁)
+  let ty₂ := .option (.ext xty₂)
+  if arg₁.term.typeOf = ty₁ && arg₂.term.typeOf = ty₂
+  then .ok {
+    term := ifSome arg₁.term (ifSome arg₂.term (enc (option.get arg₁.term) (option.get arg₂.term)))
+    footprint := arg₁.footprint ∪ arg₂.footprint
+  }
+  else .error .typeError
+
+def compileCall₂ (xty : ExtType) (enc : Term → Term → Term) (arg₁ arg₂ : CompileResult) : Result CompileResult :=
+  compileCallWithError₂ xty xty (λ t₁ t₂ => ⊙ enc t₁ t₂) arg₁ arg₂
+
+def compileCall (xfn : ExtFun) (args : List CompileResult) : Result CompileResult := do
+  match xfn, args with
+  | .decimal, [t₁]                => compileCall₀ Ext.Decimal.decimal t₁
+  | .lessThan, [t₁, t₂]           => compileCall₂ .decimal Decimal.lessThan t₁ t₂
+  | .lessThanOrEqual, [t₁, t₂]    => compileCall₂ .decimal Decimal.lessThanOrEqual t₁ t₂
+  | .greaterThan, [t₁, t₂]        => compileCall₂ .decimal Decimal.greaterThan t₁ t₂
+  | .greaterThanOrEqual, [t₁, t₂] => compileCall₂ .decimal Decimal.greaterThanOrEqual t₁ t₂
+  | .ip, [t₁]                     => compileCall₀ Ext.IPAddr.ip t₁
+  | .isIpv4, [t₁]                 => compileCall₁ .ipAddr IPAddr.isIpv4 t₁
+  | .isIpv6, [t₁]                 => compileCall₁ .ipAddr IPAddr.isIpv6 t₁
+  | .isLoopback, [t₁]             => compileCall₁ .ipAddr IPAddr.isLoopback t₁
+  | .isMulticast, [t₁]            => compileCall₁ .ipAddr IPAddr.isMulticast t₁
+  | .isInRange, [t₁, t₂]          => compileCall₂ .ipAddr IPAddr.isInRange t₁ t₂
+  | .datetime, [t₁]               => compileCall₀ Ext.Datetime.datetime t₁
+  | .duration, [t₁]               => compileCall₀ Ext.Datetime.duration t₁
+  | .offset, [t₁, t₂]             => compileCallWithError₂ .datetime .duration Datetime.offset t₁ t₂
+  | .durationSince, [t₁, t₂]      => compileCallWithError₂ .datetime .datetime Datetime.durationSince t₁ t₂
+  | .toDate, [t₁]                 => compileCallWithError₁ .datetime Datetime.toDate t₁
+  | .toTime, [t₁]                 => compileCall₁ .datetime Datetime.toTime t₁
+  | .toMilliseconds, [t₁]         => compileCall₁ .duration Duration.toMilliseconds t₁
+  | .toSeconds, [t₁]              => compileCall₁ .duration Duration.toSeconds t₁
+  | .toMinutes, [t₁]              => compileCall₁ .duration Duration.toMinutes t₁
+  | .toHours, [t₁]                => compileCall₁ .duration Duration.toHours t₁
+  | .toDays, [t₁]                 => compileCall₁ .duration Duration.toDays t₁
+  | _, _                          => .error .typeError
+
+/--
+Given an expression `x` that has type `τ` with respect to a type environment
+`Γ`, and given a well-formed symbolic environment `εnv` that conforms to `Γ`,
+`compile x εnv` succeeds and produces a well-formed term of type `.option τ.toTermType`.
+-/
+def compile (x : Expr) (εnv : SymEnv) : Result CompileResult := do
+  match x with
+  | .lit l => compilePrim l εnv.entities
+  | .var v => compileVar v εnv.request
+  | .ite x₁ x₂ x₃ =>
+    compileIf (← compile x₁ εnv) (compile x₂ εnv) (compile x₃ εnv)
+  | .and x₁ x₂ =>
+    compileAnd (← compile x₁ εnv) (compile x₂ εnv)
+  | .or x₁ x₂ =>
+    compileOr (← compile x₁ εnv) (compile x₂ εnv)
+  | .unaryApp op₁ x₁ =>
+    let res₁ ← compile x₁ εnv
+    let res ← compileApp₁ op₁ (res₁.mapTerm option.get)
+    res.mapTerm (ifSome res₁.term ·)
+  | .binaryApp op₂ x₁ x₂ =>
+    let res₁ ← compile x₁ εnv
+    let res₂ ← compile x₂ εnv
+    -- subtlety:
+    -- the unoptimized _compiler_ calls `option.get` on the terms passed to `compileApp₂`,
+    -- similar to how it's done for `compileApp₁`, `compileHasAttr`, etc.
+    -- However, for _footprint_ purposes, the unoptimized `footprint` function expresses
+    -- the footprint in terms of the original terms, without the `option.get`.
+    -- In order to give our optimized `compileApp₂` easy access to both the original and
+    -- `option.get` terms, we pass the original ones here.
+    let res ← compileApp₂ op₂ res₁ res₂ εnv.entities
+    res.mapTerm λ term => (ifSome res₁.term (ifSome res₂.term term))
+  | .hasAttr x a =>
+    let res₁ ← compile x εnv
+    let res ← compileHasAttr (res₁.mapTerm option.get) a εnv.entities
+    res.mapTerm (ifSome res₁.term ·)
+  | .getAttr x a =>
+    -- subtlety:
+    -- similar to the comment above in the `binaryApp` case
+    let res₁ ← compile x εnv
+    let res ← compileGetAttr res₁ a εnv.entities
+    res.mapTerm (ifSome res₁.term ·)
+  | .set xs =>
+    let ress ← xs.mapM₁ (λ ⟨x₁, _⟩ => compile x₁ εnv)
+    compileSet ress
+  | .record axs =>
+    let ats ← axs.mapM₂ (λ ⟨(a₁, x₁), _⟩ => do .ok (a₁, ← compile x₁ εnv))
+    compileRecord ats
+  | .call xfn xs =>
+    let ress ← xs.mapM₁ (λ ⟨x₁, _⟩ => compile x₁ εnv)
+    compileCall xfn ress
+
+namespace Cedar.SymCC
