cedar-lean/Cedar/Thm/SymCC/Opt/Compiler.lean
@@ -1,0 +1,1133 @@
+/-
+ Copyright Cedar Contributors
+
+ Licensed under the Apache License, Version 2.0 (the "License");
+ you may not use this file except in compliance with the License.
+ You may obtain a copy of the License at
+
+      https://www.apache.org/licenses/LICENSE-2.0
+
+ Unless required by applicable law or agreed to in writing, software
+ distributed under the License is distributed on an "AS IS" BASIS,
+ WITHOUT WARRANTIES OR CONDITIONS OF ANY KIND, either express or implied.
+ See the License for the specific language governing permissions and
+ limitations under the License.
+-/
+
+import Cedar.SymCC.Enforcer
+import Cedar.SymCCOpt.Compiler
+import Cedar.Thm.SymbolicCompilation
+import Cedar.Thm.SymCC.Data.LT
+import Cedar.Thm.SymCC.Enforcer.Footprint
+
+namespace Cedar.Thm
+
+open Cedar Spec SymCC
+open Cedar.Validation (ExtType)
+
+/--
+Helper lemma
+-/
+private theorem Opt.directFootprint.correctness {x : Expr} {εnv : SymEnv} {t : Term} :
+  SymCC.compile x εnv = .ok t →
+  Opt.directFootprint t = footprint.ofEntity x εnv
+:= by
+  intro h
+  simp [Opt.directFootprint, footprint.ofEntity, h]
+
+/--
+Helper lemma
+-/
+private theorem Opt.directFootprint.someFalse :
+  Opt.directFootprint (⊙false) = ∅
+:= by
+  simp [EmptyCollection.emptyCollection, Opt.directFootprint, Factory.someOf, Term.typeOf, TermPrim.typeOf, TermType.isOptionEntityType]
+
+/--
+Correctness lemma for `Opt.compileApp₁`, at least as to the `term`:
+`Opt.compileApp₁` produces the same `term` as `SymCC.compileApp₁`
+-/
+private theorem Opt.compileApp₁.correctness (op : UnaryOp) (term : Term) (footprint : Data.Set Term) :
+  Opt.compileApp₁ op { term, footprint } =
+  (do let term ← SymCC.compileApp₁ op term ; .ok { term, footprint })
+:= by
+  cases op <;> simp only [Opt.compileApp₁, SymCC.compileApp₁]
+  all_goals split <;> simp_all [Opt.CompileResult.mapTerm]
+
+/--
+Correctness lemma for `Opt.compileApp₂`, at least as to the `term`:
+`Opt.compileApp₂` produces the same `term` as `SymCC.compileApp₂`
+
+This theorem has to be adjusted for the fact that `SymCC.compileApp₂`
+expects arguments that have `option.get` applied, while `Opt.compileApp₂`
+does not. See detailed note in `Opt.compile`.
+-/
+private theorem Opt.compileApp₂.correctness (op : BinaryOp) (t₁ t₂ : Term) (ft₁ ft₂ : Data.Set Term) (εs : SymEntities) :
+  Opt.compileApp₂ op
+    { term := t₁, footprint := ft₁ }
+    { term := t₂, footprint := ft₂ }
+    εs =
+  (do
+    let term ← SymCC.compileApp₂ op (Factory.option.get t₁) (Factory.option.get t₂) εs
+    let footprint := ft₁ ∪ ft₂ ∪ Opt.directFootprint (Factory.ifSome t₁ (Factory.ifSome t₂ term))
+    .ok { term, footprint }
+  )
+:= by
+  cases op <;> simp only [Opt.compileApp₂, SymCC.compileApp₂]
+  case eq =>
+    cases reducibleEq (Factory.option.get t₁).typeOf (Factory.option.get t₂).typeOf <;> simp
+    case ok b => cases b <;> simp
+  case getTag | hasTag =>
+    split <;> simp at *
+    split <;> simp_all
+  case mem | less | lessEq | add | sub | mul =>
+    split <;> simp_all
+  case contains | containsAll | containsAny =>
+    split <;> simp at *
+    split <;> simp_all
+
+/--
+Correctness lemma for `Opt.compileGetAttr`, at least as to the `term`:
+`Opt.compileGetAttr` produces the same `term` as `SymCC.compileGetAttr`
+
+This theorem has to be adjusted for the fact that `SymCC.compileGetAttr`
+expects arguments that have `option.get` applied, while `Opt.compileGetAttr`
+does not. See detailed note in `Opt.compile`.
+-/
+private theorem Opt.compileGetAttr.correctness (t₁ : Term) (attr : Attr) (εs : SymEntities) (footprint : Data.Set Term) :
+  Opt.compileGetAttr { term := t₁, footprint } attr εs =
+  (do let term ← SymCC.compileGetAttr (Factory.option.get t₁) attr εs ; .ok { term, footprint := footprint ∪ Opt.directFootprint (Factory.ifSome t₁ term) })
+:= by
+  simp only [Opt.compileGetAttr, SymCC.compileGetAttr, Except.bind_ok, Except.bind_err, bind_assoc]
+  simp_do_let compileAttrsOf (Factory.option.get t₁) εs
+  split <;> rename_i h <;> simp [h]
+  split <;> rename_i h <;> simp [h]
+  all_goals apply Data.Set.union_comm
+
+/--
+Correctness lemma for `Opt.compileHasAttr`, at least as to the `term`:
+`Opt.compileHasAttr` produces the same `term` as `SymCC.compileHasAttr`
+-/
+private theorem Opt.compileHasAttr.correctness (t₁ : Term) (attr : Attr) (εs : SymEntities) (footprint : Data.Set Term) :
+  Opt.compileHasAttr { term := t₁, footprint } attr εs =
+  (do let term ← SymCC.compileHasAttr t₁ attr εs ; .ok { term, footprint })
+:= by
+  simp only [Opt.compileHasAttr, SymCC.compileHasAttr, bind_assoc]
+  simp_do_let compileAttrsOf t₁ εs ; rename_i h₁
+  split <;> rename_i h <;> simp [h]
+  split <;> rename_i h <;> simp [h]
+
+/--
+Correctness lemma for `Opt.compileSet`, at least as to the `term`:
+`Opt.compileSet` produces the same `term` as `SymCC.compileSet`
+-/
+private theorem Opt.compileSet.correctness (ress : List Opt.CompileResult) :
+  Opt.compileSet ress =
+  (do let term ← SymCC.compileSet (ress.map Opt.CompileResult.term) ; .ok { term, footprint := ress.mapUnion Opt.CompileResult.footprint })
+:= by
+  simp only [Opt.compileSet, SymCC.compileSet, List.all_map, List.all_eq_true, Function.comp_apply,
+    decide_eq_true_eq, List.map_map]
+  cases ress
+  case nil => simp
+  case cons hd tl =>
+    simp only [List.mem_cons, forall_eq_or_imp, List.map_cons, Function.comp_apply]
+    split <;> rename_i hhd <;> simp [hhd]
+    split <;> rename_i htl <;> simp
+
+/--
+Correctness lemma for `Opt.compileRecord`, at least as to the `term`:
+`Opt.compileRecord` produces the same `term` as `SymCC.compileRecord`
+-/
+private theorem Opt.compileRecord.correctness (ress : List (Attr × Opt.CompileResult)) :
+  Opt.compileRecord ress =
+  {
+    term := SymCC.compileRecord (ress.map λ (a, res) => (a, res.term))
+    footprint := ress.mapUnion λ (_, res) => res.footprint
+  }
+:= by
+  simp only [Opt.compileRecord, SymCC.compileRecord, List.map_map, Opt.CompileResult.mk.injEq, and_true]
+  cases ress
+  case nil => simp
+  case cons hd tl =>
+    simp only [List.map_cons, Function.comp_apply, Prod.map_apply, id_eq]
+    congr
+
+/--
+Correctness lemma for `Opt.compileCall₀`, at least as to the `term`:
+`Opt.compileCall₀` produces the same `term` as `SymCC.compileCall₀`
+-/
+private theorem Opt.compileCall₀.correctness {α} [Coe α Ext] (mk : String → Option α) (res : Opt.CompileResult) :
+  Opt.compileCall₀ mk res =
+  (do let term ← SymCC.compileCall₀ mk res.term ; .ok { term, footprint := res.footprint })
+:= by
+  simp only [Opt.compileCall₀, compileCall₀]
+  split
+  · split <;> rename_i hs <;> simp [hs]
+  · symm ; rw [do_error]
+    split
+    · exfalso
+      rename_i h₁ t s h₂
+      apply h₁ s res.footprint ; clear h₁
+      cases res ; simp_all
+    · rfl
+
+/--
+Correctness lemma for `Opt.compileCallWithError₁`, at least as to the `term`:
+`Opt.compileCall₁` produces the same `term` as `SymCC.compileCallWithError₁`
+-/
+private theorem Opt.compileCallWithError₁.correctness (xty : ExtType) (enc : Term → Term) (res : Opt.CompileResult) :
+  Opt.compileCallWithError₁ xty enc res =
+  (do let term ← SymCC.compileCallWithError₁ xty enc res.term ; .ok { term, footprint := res.footprint })
+:= by
+  simp only [Opt.compileCallWithError₁, compileCallWithError₁]
+  split <;> simp
+
+/--
+Correctness lemma for `Opt.compileCall₁`, at least as to the `term`:
+`Opt.compileCall₁` produces the same `term` as `SymCC.compileCall₁`
+-/
+private theorem Opt.compileCall₁.correctness (xty : ExtType) (enc : Term → Term) (res : Opt.CompileResult) :
+  Opt.compileCall₁ xty enc res =
+  (do let term ← SymCC.compileCall₁ xty enc res.term ; .ok { term, footprint := res.footprint })
+:= by
+  simp only [Opt.compileCall₁, SymCC.compileCall₁]
+  rw [Opt.compileCallWithError₁.correctness]
+
+/--
+Correctness lemma for `Opt.compileCallWithError₂`, at least as to the `term`:
+`Opt.compileCallWithError₂` produces the same `term` as `SymCC.compileCallWithError₂`
+-/
+private theorem Opt.compileCallWithError₂.correctness (xty₁ xty₂ : ExtType) (enc : Term → Term → Term) (res₁ res₂ : Opt.CompileResult) :
+  Opt.compileCallWithError₂ xty₁ xty₂ enc res₁ res₂ =
+  (do let term ← SymCC.compileCallWithError₂ xty₁ xty₂ enc res₁.term res₂.term ; .ok { term, footprint := res₁.footprint ∪ res₂.footprint })
+:= by
+  simp only [Opt.compileCallWithError₂, SymCC.compileCallWithError₂]
+  split <;> simp
+
+/--
+Correctness lemma for `Opt.compileCall₂`, at least as to the `term`:
+`Opt.compileCall₂` produces the same `term` as `SymCC.compileCall₂`
+-/
+private theorem Opt.compileCall₂.correctness (xty : ExtType) (enc : Term → Term → Term) (res₁ res₂ : Opt.CompileResult) :
+  Opt.compileCall₂ xty enc res₁ res₂ =
+  (do let term ← SymCC.compileCall₂ xty enc res₁.term res₂.term ; .ok { term, footprint := res₁.footprint ∪ res₂.footprint })
+:= by
+  simp only [Opt.compileCall₂, SymCC.compileCall₂]
+  rw [Opt.compileCallWithError₂.correctness]
+
+/--
+Correctness lemma for `Opt.compileCall`, at least as to the `term`:
+`Opt.compileCall` produces the same `term` as `SymCC.compileCall`
+-/
+private theorem Opt.compileCall.correctness (xfn : ExtFun) (ress : List Opt.CompileResult)
+  (hwf : ∀ res ∈ ress, res.footprint.WellFormed) :
+  Opt.compileCall xfn ress =
+  (do let term ← SymCC.compileCall xfn (ress.map Opt.CompileResult.term) ; .ok { term, footprint := ress.mapUnion Opt.CompileResult.footprint })
+:= by
+  simp only [Opt.compileCall, SymCC.compileCall]
+  split <;> try simp only [Opt.compileCall₀.correctness, Opt.compileCall₁.correctness, Opt.compileCall₂.correctness, List.map_cons, List.map_nil]
+  all_goals first
+  | simp only [Opt.compileCall₀.correctness] | simp only [Opt.compileCall₁.correctness] | simp only [Opt.compileCall₂.correctness] | simp only [Opt.compileCallWithError₁.correctness] | simp only [Opt.compileCallWithError₂.correctness] | symm
+  · rename_i res ; simp_do_let SymCC.compileCall₀ Ext.Decimal.decimal res.term
+    rw [Data.Set.mapUnion_singleton (by apply hwf res (by simp))]
+  · rename_i res₁ res₂ ; simp_do_let SymCC.compileCall₂ _ Decimal.lessThan res₁.term res₂.term
+    rw [Data.Set.mapUnion_cons hwf]
+    rw [Data.Set.mapUnion_singleton (by apply hwf res₂ (by simp))]
+  · rename_i res₁ res₂ ; simp_do_let SymCC.compileCall₂ _ Decimal.lessThanOrEqual res₁.term res₂.term
+    rw [Data.Set.mapUnion_cons hwf]
+    rw [Data.Set.mapUnion_singleton (by apply hwf res₂ (by simp))]
+  · rename_i res₁ res₂ ; simp_do_let SymCC.compileCall₂ _ Decimal.greaterThan res₁.term res₂.term
+    rw [Data.Set.mapUnion_cons hwf]
+    rw [Data.Set.mapUnion_singleton (by apply hwf res₂ (by simp))]
+  · rename_i res₁ res₂ ; simp_do_let SymCC.compileCall₂ _ Decimal.greaterThanOrEqual res₁.term res₂.term
+    rw [Data.Set.mapUnion_cons hwf]
+    rw [Data.Set.mapUnion_singleton (by apply hwf res₂ (by simp))]
+  · rename_i res ; simp_do_let SymCC.compileCall₀ Ext.IPAddr.ip res.term
+    rw [Data.Set.mapUnion_singleton (by apply hwf res (by simp))]
+  · rename_i res ; simp_do_let SymCC.compileCall₁ _ IPAddr.isIpv4 res.term
+    rw [Data.Set.mapUnion_singleton (by apply hwf res (by simp))]
+  · rename_i res ; simp_do_let SymCC.compileCall₁ _ IPAddr.isIpv6 res.term
+    rw [Data.Set.mapUnion_singleton (by apply hwf res (by simp))]
+  · rename_i res ; simp_do_let SymCC.compileCall₁ _ IPAddr.isLoopback res.term
+    rw [Data.Set.mapUnion_singleton (by apply hwf res (by simp))]
+  · rename_i res ; simp_do_let SymCC.compileCall₁ _ IPAddr.isMulticast res.term
+    rw [Data.Set.mapUnion_singleton (by apply hwf res (by simp))]
+  · rename_i res₁ res₂ ; simp_do_let SymCC.compileCall₂ _ IPAddr.isInRange res₁.term res₂.term
+    rw [Data.Set.mapUnion_cons hwf]
+    rw [Data.Set.mapUnion_singleton (by apply hwf res₂ (by simp))]
+  · rename_i res ; simp_do_let SymCC.compileCall₀ Ext.Datetime.datetime res.term
+    rw [Data.Set.mapUnion_singleton (by apply hwf res (by simp))]
+  · rename_i res ; simp_do_let SymCC.compileCall₀ Ext.Datetime.duration res.term
+    rw [Data.Set.mapUnion_singleton (by apply hwf res (by simp))]
+  · rename_i res₁ res₂ ; simp_do_let SymCC.compileCallWithError₂ _ _ Datetime.offset res₁.term res₂.term
+    rw [Data.Set.mapUnion_cons hwf]
+    rw [Data.Set.mapUnion_singleton (by apply hwf res₂ (by simp))]
+  · rename_i res₁ res₂ ; simp_do_let SymCC.compileCallWithError₂ _ _ Datetime.durationSince res₁.term res₂.term
+    rw [Data.Set.mapUnion_cons hwf]
+    rw [Data.Set.mapUnion_singleton (by apply hwf res₂ (by simp))]
+  · rename_i res ; simp_do_let SymCC.compileCallWithError₁ _ Datetime.toDate res.term
+    rw [Data.Set.mapUnion_singleton (by apply hwf res (by simp))]
+  · rename_i res ; simp_do_let SymCC.compileCall₁ _ Datetime.toTime res.term
+    rw [Data.Set.mapUnion_singleton (by apply hwf res (by simp))]
+  · rename_i res ; simp_do_let SymCC.compileCall₁ _ Duration.toMilliseconds res.term
+    rw [Data.Set.mapUnion_singleton (by apply hwf res (by simp))]
+  · rename_i res ; simp_do_let SymCC.compileCall₁ _ Duration.toSeconds res.term
+    rw [Data.Set.mapUnion_singleton (by apply hwf res (by simp))]
+  · rename_i res ; simp_do_let SymCC.compileCall₁ _ Duration.toMinutes res.term
+    rw [Data.Set.mapUnion_singleton (by apply hwf res (by simp))]
+  · rename_i res ; simp_do_let SymCC.compileCall₁ _ Duration.toHours res.term
+    rw [Data.Set.mapUnion_singleton (by apply hwf res (by simp))]
+  · rename_i res ; simp_do_let SymCC.compileCall₁ _ Duration.toDays res.term
+    rw [Data.Set.mapUnion_singleton (by apply hwf res (by simp))]
+  · rw [do_error]
+    split <;> simp_all
+    all_goals {
+      rename_i t₁ t₂ h₁ h₂
+      have ⟨res₁, res₂, hres⟩ := List.map_eq_doubleton h₁
+      specialize h₂ res₁ res₂ ; contradiction
+    }
+
+/--
+Helper lemma that `Opt.compileCall₀` produces a well-formed footprint set.
+-/
+private theorem Opt.compileCall₀_footprint_wf [Coe α Ext] {mk : String → Option α} {term : Term} {footprint : Data.Set Term} {res : Opt.CompileResult} :
+  footprint.WellFormed →
+  Opt.compileCall₀ mk { term, footprint } = .ok res →
+  res.footprint.WellFormed
+:= by
+  simp [Opt.compileCall₀]
+  split <;> rename_i h
+  · simp at h ; replace ⟨h, h'⟩ := h ; subst term footprint
+    split <;> simp
+    intro wf h ; subst res ; simp [wf]
+  · simp
+
+/--
+Helper lemma that `Opt.compileCallWithError₁` produces a well-formed footprint set.
+-/
+private theorem Opt.compileCallWithError₁_footprint_wf {xty : ExtType} {arg res : Opt.CompileResult} :
+  arg.footprint.WellFormed →
+  Opt.compileCallWithError₁ xty enc arg = .ok res →
+  res.footprint.WellFormed
+:= by
+  simp [Opt.compileCallWithError₁]
+  split <;> simp
+  intro wf h ; subst res ; simp [wf]
+
+/--
+Helper lemma that `Opt.compileCall₁` produces a well-formed footprint set.
+-/
+private theorem Opt.compileCall₁_footprint_wf {xty : ExtType} {arg res : Opt.CompileResult} :
+  arg.footprint.WellFormed →
+  Opt.compileCall₁ xty enc arg = .ok res →
+  res.footprint.WellFormed
+:= by
+  unfold Opt.compileCall₁
+  exact Opt.compileCallWithError₁_footprint_wf
+
+/--
+Helper lemma that `Opt.compileCallWithError₂` produces a well-formed footprint set.
+
+Unlike the ₀ and ₁ cases, this case does not require that the args are well-formed.
+-/
+private theorem Opt.compileCallWithError₂_footprint_wf {xty₁ xty₂ : ExtType} {arg₁ arg₂ res : Opt.CompileResult} :
+  Opt.compileCallWithError₂ xty₁ xty₂ enc arg₁ arg₂ = .ok res →
+  res.footprint.WellFormed
+:= by
+  simp [Opt.compileCallWithError₂]
+  split <;> simp
+  intro h ; subst res ; simp [Data.Set.union_wf]
+
+/--
+Helper lemma that `Opt.compileCall₂` produces a well-formed footprint set.
+
+Unlike the ₀ and ₁ cases, this case does not require that the args are well-formed.
+-/
+private theorem Opt.compileCall₂_footprint_wf {xty : ExtType} {arg₁ arg₂ res : Opt.CompileResult} :
+  Opt.compileCall₂ xty enc arg₁ arg₂ = .ok res →
+  res.footprint.WellFormed
+:= by
+  unfold Opt.compileCall₂
+  exact Opt.compileCallWithError₂_footprint_wf
+
+/--
+Lemma that `Opt.compile` produces a well-formed footprint set.
+-/
+theorem Opt.compile_footprint_wf {x : Expr} {εnv : SymEnv} {res : Opt.CompileResult} :
+  Opt.compile x εnv = .ok res →
+  res.footprint.WellFormed
+:= by
+  cases x <;> simp [Opt.compile]
+  case lit p =>
+    cases p <;> simp [Opt.compilePrim]
+    case bool | int | string =>
+      intro h ; subst res ; simp [EmptyCollection.emptyCollection, Data.Set.empty_wf]
+    case entityUID =>
+      split <;> simp
+      · intro h ; subst res ; simp [Data.Set.singleton_wf]
+  case var v =>
+    cases v <;> simp [Opt.compileVar] <;> split <;> simp
+    · intro h ; subst res ; simp [Data.Set.singleton_wf]
+    · intro h ; subst res ; simp [Data.Set.singleton_wf]
+    · intro h ; subst res ; simp [Data.Set.singleton_wf]
+    · intro h ; subst res ; simp [EmptyCollection.emptyCollection, Data.Set.empty_wf]
+  case ite x₁ x₂ x₃ =>
+    simp_do_let Opt.compile x₁ εnv
+    case error => simp
+    case ok =>
+      simp [Opt.compileIf]
+      split
+      · exact Opt.compile_footprint_wf
+      · exact Opt.compile_footprint_wf
+      · simp_do_let Opt.compile x₂ εnv
+        case error => simp
+        case ok =>
+          simp_do_let Opt.compile x₃ εnv
+          case error => simp
+          case ok =>
+            split <;> simp
+            intro h ; subst res ; simp [Data.Set.union_wf]
+      · simp
+  case and x₁ x₂ | or x₁ x₂ =>
+    simp_do_let Opt.compile x₁ εnv
+    case error => simp
+    case ok =>
+      rename_i res' h₁
+      simp [Opt.compileAnd, Opt.compileOr]
+      split
+      · simp ; intro h ; subst res ; simp [EmptyCollection.emptyCollection, Data.Set.empty_wf]
+      · simp_do_let Opt.compile x₂ εnv
+        case error => simp
+        case ok =>
+          split <;> simp
+          intro h ; subst res ; simp
+          split
+          · apply Opt.compile_footprint_wf ; assumption
+          · simp [Data.Set.union_wf]
+      · simp
+  case unaryApp op x₁ =>
+    simp_do_let Opt.compile x₁ εnv
+    case error => simp
+    case ok res₁ =>
+      simp_do_let Opt.compileApp₁ op _
+      case error => simp
+      case ok resApp _ =>
+        simp ; intro h ; subst res
+        simp [Opt.CompileResult.mapTerm]
+        -- we could make the remainder of this case a separate lemma `Opt.compileApp₁_footprint_wf`, but leaving it inline for now
+        rename_i h₁ ; revert h₁
+        simp [Opt.compileApp₁]
+        split <;> simp
+        all_goals {
+          intro h ; subst resApp
+          simp [Opt.CompileResult.mapTerm]
+          apply Opt.compile_footprint_wf ; assumption
+        }
+  case binaryApp op x₁ x₂ =>
+    simp_do_let Opt.compile x₁ εnv
+    case error => simp
+    case ok res₁ h₁ =>
+      simp_do_let Opt.compile x₂ εnv
+      case error => simp
+      case ok res₂ h₂ =>
+        simp_do_let Opt.compileApp₂ op res₁ res₂ εnv.entities
+        case error => simp
+        case ok resApp h₃ =>
+          simp ; intro h ; subst res
+          simp [Opt.CompileResult.mapTerm]
+          -- we could make the remainder of this case a separate lemma `Opt.compileApp₂_footprint_wf`, but leaving it inline for now
+          revert h₃
+          simp [Opt.compileApp₂]
+          split
+          · simp_do_let reducibleEq _ _
+            case error => simp
+            case ok b hb =>
+              simp ; intro h ; subst resApp ; simp [Data.Set.union_wf]
+          · simp ; intro h ; subst resApp ; simp [Data.Set.union_wf]
+          · simp ; intro h ; subst resApp ; simp [Data.Set.union_wf]
+          · simp ; intro h ; subst resApp ; simp [Data.Set.union_wf]
+          · simp ; intro h ; subst resApp ; simp [Data.Set.union_wf]
+          · simp ; intro h ; subst resApp ; simp [Data.Set.union_wf]
+          · simp ; intro h ; subst resApp ; simp [Data.Set.union_wf]
+          · simp ; intro h ; subst resApp ; simp [Data.Set.union_wf]
+          · simp ; intro h ; subst resApp ; simp [Data.Set.union_wf]
+          · simp ; intro h ; subst resApp ; simp [Data.Set.union_wf]
+          · split <;> simp
+            intro h ; subst resApp ; simp [Data.Set.union_wf]
+          · split <;> simp
+            intro h ; subst resApp ; simp [Data.Set.union_wf]
+          · split <;> simp
+            intro h ; subst resApp ; simp [Data.Set.union_wf]
+          · simp ; intro h ; subst resApp ; simp [Data.Set.union_wf]
+          · simp ; intro h ; subst resApp ; simp [Data.Set.union_wf]
+          · simp_do_let compileHasTag _ _ _
+            case error => simp
+            case ok => simp ; intro h ; subst resApp ; simp [Data.Set.union_wf]
+          · simp_do_let compileGetTag _ _ _
+            case error => simp
+            case ok => simp ; intro h ; subst resApp ; simp [Data.Set.union_wf]
+          · simp
+  case hasAttr x₁ attr =>
+    simp_do_let Opt.compile x₁ εnv
+    case error => simp
+    case ok res₁ h₁ =>
+      simp_do_let Opt.compileHasAttr _ _ _
+      case error => simp
+      case ok res₂ h₂ =>
+        simp ; intro h ; subst res
+        simp [Opt.CompileResult.mapTerm]
+        -- we could make the remainder of this case a separate lemma `Opt.compileHasAttr_footprint_wf`, but leaving it inline for now
+        revert h₂
+        simp [Opt.compileHasAttr]
+        simp_do_let compileAttrsOf _ _
+        case error => simp
+        case ok t ht =>
+          split
+          · split <;> simp
+            all_goals {
+              intro h ; subst res₂
+              simp [Opt.CompileResult.mapTerm]
+              exact Opt.compile_footprint_wf h₁
+            }
+          · simp
+  case getAttr x₁ attr =>
+    simp_do_let Opt.compile x₁ εnv
+    case error => simp
+    case ok res₁ h₁ =>
+      simp_do_let Opt.compileGetAttr res₁ attr εnv.entities
+      case error => simp
+      case ok res₂ h₂ =>
+        simp ; intro h ; subst res
+        simp [Opt.CompileResult.mapTerm]
+        -- we could make the remainder of this case a separate lemma `Opt.compileGetAttr_footprint_wf`, but leaving it inline for now
+        revert h₂
+        simp [Opt.compileGetAttr]
+        simp_do_let compileAttrsOf _ _
+        case error => simp
+        case ok t ht =>
+          split
+          · split <;> simp
+            all_goals {
+              intro h ; subst res₂ ; simp [Data.Set.union_wf]
+            }
+          · simp
+  case set xs =>
+    rw [List.mapM₁_eq_mapM (Opt.compile · εnv)]
+    simp_do_let xs.mapM (Opt.compile · εnv)
+    case error => simp
+    case ok ress hress =>
+      -- we could make the remainder of this case a separate lemma `Opt.compileSet_footprint_wf`, but leaving it inline for now
+      simp [Opt.compileSet]
+      split
+      · simp
+      · split
+        · split <;> simp
+          intro h ; subst res ; simp [Data.Set.mapUnion_wf]
+        · simp
+  case record axs =>
+    rw [do_eq_ok]
+    intro h ; replace ⟨aress, haress, h⟩ := h
+    simp at h ; subst res
+    -- we could make the remainder of this case a separate lemma `Opt.compileRecord_footprint_wf`, but leaving it inline for now
+    simp [Opt.compileRecord, Data.Set.mapUnion_wf]
+  case call xfn args =>
+    rw [List.mapM₁_eq_mapM (Opt.compile · εnv)]
+    simp_do_let args.mapM (Opt.compile · εnv)
+    case error => simp
+    case ok ress hress =>
+      -- we could make the remainder of this case a separate lemma `Opt.compileCall_footprint_wf`, but leaving it inline for now
+      simp [Opt.compileCall]
+      replace hress := List.mapM_ok_implies_all_from_ok hress
+      split
+      · apply Opt.compileCall₀_footprint_wf
+        rename_i res'
+        have ⟨arg, harg, h₁⟩ := hress res' (by simp)
+        exact Opt.compile_footprint_wf h₁
+      · exact Opt.compileCall₂_footprint_wf
+      · exact Opt.compileCall₂_footprint_wf
+      · exact Opt.compileCall₂_footprint_wf
+      · exact Opt.compileCall₂_footprint_wf
+      · apply Opt.compileCall₀_footprint_wf
+        rename_i res'
+        have ⟨arg, harg, h₁⟩ := hress res' (by simp)
+        exact Opt.compile_footprint_wf h₁
+      · apply Opt.compileCall₁_footprint_wf
+        rename_i res'
+        have ⟨arg, harg, h₁⟩ := hress res' (by simp)
+        exact Opt.compile_footprint_wf h₁
+      · apply Opt.compileCall₁_footprint_wf
+        rename_i res'
+        have ⟨arg, harg, h₁⟩ := hress res' (by simp)
+        exact Opt.compile_footprint_wf h₁
+      · apply Opt.compileCall₁_footprint_wf
+        rename_i res'
+        have ⟨arg, harg, h₁⟩ := hress res' (by simp)
+        exact Opt.compile_footprint_wf h₁
+      · apply Opt.compileCall₁_footprint_wf
+        rename_i res'
+        have ⟨arg, harg, h₁⟩ := hress res' (by simp)
+        exact Opt.compile_footprint_wf h₁
+      · exact Opt.compileCall₂_footprint_wf
+      · apply Opt.compileCall₀_footprint_wf
+        rename_i res'
+        have ⟨arg, harg, h₁⟩ := hress res' (by simp)
+        exact Opt.compile_footprint_wf h₁
+      · apply Opt.compileCall₀_footprint_wf
+        rename_i res'
+        have ⟨arg, harg, h₁⟩ := hress res' (by simp)
+        exact Opt.compile_footprint_wf h₁
+      · exact Opt.compileCallWithError₂_footprint_wf
+      · exact Opt.compileCallWithError₂_footprint_wf
+      · apply Opt.compileCallWithError₁_footprint_wf
+        rename_i res'
+        have ⟨arg, harg, h₁⟩ := hress res' (by simp)
+        exact Opt.compile_footprint_wf h₁
+      · apply Opt.compileCall₁_footprint_wf
+        rename_i res'
+        have ⟨arg, harg, h₁⟩ := hress res' (by simp)
+        exact Opt.compile_footprint_wf h₁
+      · apply Opt.compileCall₁_footprint_wf
+        rename_i res'
+        have ⟨arg, harg, h₁⟩ := hress res' (by simp)
+        exact Opt.compile_footprint_wf h₁
+      · apply Opt.compileCall₁_footprint_wf
+        rename_i res'
+        have ⟨arg, harg, h₁⟩ := hress res' (by simp)
+        exact Opt.compile_footprint_wf h₁
+      · apply Opt.compileCall₁_footprint_wf
+        rename_i res'
+        have ⟨arg, harg, h₁⟩ := hress res' (by simp)
+        exact Opt.compile_footprint_wf h₁
+      · apply Opt.compileCall₁_footprint_wf
+        rename_i res'
+        have ⟨arg, harg, h₁⟩ := hress res' (by simp)
+        exact Opt.compile_footprint_wf h₁
+      · apply Opt.compileCall₁_footprint_wf
+        rename_i res'
+        have ⟨arg, harg, h₁⟩ := hress res' (by simp)
+        exact Opt.compile_footprint_wf h₁
+      · simp
+
+/--
+Lemma pulled out from the below `mutual` block so that we can prove it on its own by induction
+without worrying about making the `mutual` block's termination proof even more complicated
+-/
+private theorem both_lists_error_then_errors_same {xs : List Expr} {εnv : SymEnv} :
+  xs.mapM (Opt.compile · εnv) = Except.error e₁ →
+  xs.mapM (SymCC.compile · εnv) = Except.error e₂ →
+  (∀ x ∈ xs, Opt.compile x εnv = (do
+    let term ← SymCC.compile x εnv
+    let footprint := footprint x εnv
+    .ok { term, footprint }
+  )) →
+  e₁ = e₂
+:= by
+  cases xs
+  case nil => simp [List.mapM_nil, pure, Except.pure]
+  case cons hd tl =>
+    simp [List.mapM_cons]
+    intro h₁ h₂ ihhd ihtl
+    rw [ihhd] at h₁
+    cases hhd : SymCC.compile hd εnv <;> simp [hhd] at h₁ h₂
+    case error e' => simp [← h₁, ← h₂]
+    case ok t =>
+      simp only [Functor.map, Except.map] at h₁
+      split at h₁ <;> simp only [Except.error.injEq, reduceCtorEq] at h₁
+      rename_i e' htl₁
+      subst e'
+      simp only [Functor.map, Except.map] at h₂
+      split at h₂ <;> simp only [Except.error.injEq, reduceCtorEq] at h₂
+      rename_i e' htl₂
+      subst e'
+      exact both_lists_error_then_errors_same htl₁ htl₂ ihtl
+
+/--
+Lemma pulled out from the below `mutual` block so that we can prove it on its own by induction
+without worrying about making the `mutual` block's termination proof even more complicated
+-/
+private theorem both_lists_pairs_error_then_errors_same {xs : List (Attr × Expr)} {εnv : SymEnv} :
+  xs.mapM (λ pair => do .ok (pair.fst, ← Opt.compile pair.snd εnv)) = Except.error e₁ →
+  xs.mapM (λ pair => do .ok (pair.fst, ← SymCC.compile pair.snd εnv)) = Except.error e₂ →
+  (∀ pair ∈ xs, Opt.compile pair.snd εnv = (do
+    let term ← SymCC.compile pair.snd εnv
+    let footprint := footprint pair.snd εnv
+    .ok { term, footprint }
+  )) →
+  e₁ = e₂
+:= by
+  cases xs
+  case nil => simp [List.mapM_nil, pure, Except.pure]
+  case cons hd tl =>
+    simp [List.mapM_cons]
+    intro h₁ h₂ ihhd ihtl
+    rw [ihhd] at h₁
+    cases hhd : SymCC.compile hd.snd εnv <;> simp [hhd] at h₁ h₂
+    case error e' => simp [← h₁, ← h₂]
+    case ok t =>
+      simp only [Functor.map, Except.map] at h₁
+      split at h₁ <;> simp only [Except.error.injEq, reduceCtorEq] at h₁
+      rename_i e' htl₁
+      subst e'
+      simp only [Functor.map, Except.map] at h₂
+      split at h₂ <;> simp only [Except.error.injEq, reduceCtorEq] at h₂
+      rename_i e' htl₂
+      subst e'
+      apply both_lists_pairs_error_then_errors_same htl₁ htl₂
+      intro pair hpair
+      exact ihtl pair.fst pair.snd hpair
+
+/--
+Lemma pulled out from the below `mutual` block so that we can prove it on its own by induction
+without worrying about making the `mutual` block's termination proof even more complicated
+-/
+private theorem both_lists_ok_then_elts_correspond {xs : List Expr} {εnv : SymEnv} :
+  xs.mapM (Opt.compile · εnv) = Except.ok ts₁ →
+  xs.mapM (SymCC.compile · εnv) = Except.ok ts₂ →
+  (∀ x ∈ xs, Opt.compile x εnv = (do
+    let term ← SymCC.compile x εnv
+    let footprint := footprint x εnv
+    .ok { term, footprint }
+  )) →
+  ts₁.map Opt.CompileResult.term = ts₂
+  ∧ ts₁.map Opt.CompileResult.footprint = xs.map (footprint · εnv)
+:= by
+  intro h₁ h₂ ih
+  cases xs
+  case nil => simp [List.mapM_nil, pure, Except.pure] at h₁ h₂ ; simp [h₁, h₂]
+  case cons hd tl =>
+    simp [List.mapM_cons, Functor.map, Except.map] at h₁ h₂
+    rw [ih _ (by simp)] at h₁
+    simp_do_let SymCC.compile hd εnv at h₁ ; rename_i hhd
+    case ok t =>
+    simp [hhd] at h₂
+    split at h₁ <;> simp at h₁
+    rename_i restl htl₁
+    subst ts₁
+    split at h₂ <;> simp at h₂
+    rename_i tstl htl₂
+    subst ts₂
+    have ⟨htemp, ih'⟩ := both_lists_ok_then_elts_correspond htl₁ htl₂ (by
+      intro x hx
+      apply ih x (by simp [hx])
+    )
+    subst tstl
+    simp [List.map_cons, ih']
+
+/--
+Lemma pulled out from the below `mutual` block so that we can prove it on its own by induction
+without worrying about making the `mutual` block's termination proof even more complicated
+-/
+private theorem both_lists_pairs_ok_then_elts_correspond {xs : List (Attr × Expr)} {εnv : SymEnv} :
+  xs.mapM (λ pair => do .ok (pair.fst, ← Opt.compile pair.snd εnv)) = Except.ok ts₁ →
+  xs.mapM (λ pair => do .ok (pair.fst, ← SymCC.compile pair.snd εnv)) = Except.ok ts₂ →
+  (∀ pair ∈ xs, Opt.compile pair.snd εnv = (do
+    let term ← SymCC.compile pair.snd εnv
+    let footprint := footprint pair.snd εnv
+    .ok { term, footprint }
+  )) →
+  ts₁.map (λ (a, res) => (a, res.term)) = ts₂
+  ∧ ts₁.map (λ (_, res) => res.footprint) = xs.map (λ (_, x) => footprint x εnv)
+:= by
+  intro h₁ h₂ ih
+  cases xs
+  case nil => simp [List.mapM_nil, pure, Except.pure] at h₁ h₂ ; simp [h₁, h₂]
+  case cons hd tl =>
+    simp [List.mapM_cons, Functor.map, Except.map] at h₁ h₂
+    rw [ih _ (by simp)] at h₁
+    simp_do_let compile hd.snd εnv at h₁ ; rename_i hhd
+    case ok t =>
+    simp [hhd] at h₂
+    split at h₁ <;> simp at h₁
+    rename_i restl htl₁
+    subst ts₁
+    split at h₂ <;> simp at h₂
+    rename_i tstl htl₂
+    subst ts₂
+    have ⟨htemp, ih'⟩ := both_lists_pairs_ok_then_elts_correspond htl₁ htl₂ (by
+      intro x hx
+      apply ih x (by simp [hx])
+    )
+    subst tstl
+    simp [List.map_cons, ih']
+
+mutual
+
+/--
+Correctness theorem for `Opt.compile` -- `lit` case
+-/
+theorem Opt.compile.correctness.lit (p : Prim) (εnv : SymEnv) :
+  Opt.compile (.lit p) εnv = (do
+    let term ← SymCC.compile (.lit p) εnv
+    let footprint := footprint (.lit p) εnv
+    .ok { term, footprint }
+  )
+:= by
+  simp [Opt.compile, SymCC.compile, footprint]
+  cases p <;> simp [Opt.compilePrim, SymCC.compilePrim, footprint.ofEntity, SymCC.compile, EmptyCollection.emptyCollection, Factory.someOf, TermType.isOptionEntityType, Term.typeOf, TermPrim.typeOf]
+  case entityUID uid => split <;> simp [Term.typeOf, TermPrim.typeOf]
+
+/--
+Correctness theorem for `Opt.compile` -- `var` case
+-/
+theorem Opt.compile.correctness.var (v : Var) (εnv : SymEnv) :
+  Opt.compile (.var v) εnv = (do
+    let term ← SymCC.compile (.var v) εnv
+    let footprint := footprint (.var v) εnv
+    .ok { term, footprint }
+  )
+:= by
+  simp [Opt.compile, SymCC.compile, footprint]
+  cases v <;> simp [Opt.compileVar, SymCC.compileVar, footprint.ofEntity, SymCC.compile, EmptyCollection.emptyCollection, Factory.someOf, TermType.isEntityType, TermType.isOptionEntityType]
+  case principal | action | resource => split <;> simp [Term.typeOf, *]
+  case context =>
+    split <;> rename_i h
+    · simp [Term.typeOf, TermType.isRecordType] at *
+      split at h <;> simp_all
+    · simp
+
+/--
+Correctness theorem for `Opt.compile` -- `ite` case
+-/
+theorem Opt.compile.correctness.ite (x₁ x₂ x₃ : Expr) (εnv : SymEnv) :
+  Opt.compile (.ite x₁ x₂ x₃) εnv = (do
+    let term ← SymCC.compile (.ite x₁ x₂ x₃) εnv
+    let footprint := footprint (.ite x₁ x₂ x₃) εnv
+    .ok { term, footprint }
+  )
+:= by
+  simp [Opt.compile, SymCC.compile, footprint]
+  rw [Opt.compile.correctness x₁ εnv, Opt.compile.correctness x₂ εnv, Opt.compile.correctness x₃ εnv]
+  simp [Opt.compileIf, SymCC.compileIf, footprint.ofBranch]
+  cases h₁ : SymCC.compile x₁ εnv <;> simp
+  case ok t₁ =>
+    split <;> simp
+    cases h₂ : SymCC.compile x₂ εnv <;> simp_all
+    case ok t₁ _ _ t₂ _ _ ht₁ =>
+      cases h₃ : SymCC.compile x₃ εnv <;> simp_all
+      case ok t₃ => split <;> simp
+termination_by 1 + 2 * sizeOf x₁ + 2 * sizeOf x₂ + 2 * sizeOf x₃
+decreasing_by all_goals {
+  have : ∀ x : Expr, sizeOf x > 0 := by
+    intro x ; cases x <;> simp [sizeOf, Expr._sizeOf_1] <;> omega
+  have hx₁ := this x₁
+  have hx₂ := this x₂
+  have hx₃ := this x₃
+  omega
+}
+
+/--
+Correctness theorem for `Opt.compile` -- `and` and `or` cases
+-/
+theorem Opt.compile.correctness.andor (x₁ x₂ : Expr) (εnv : SymEnv) :
+  Opt.compile (.and x₁ x₂) εnv = (do
+    let term ← SymCC.compile (.and x₁ x₂) εnv
+    let footprint := footprint (.and x₁ x₂) εnv
+    .ok { term, footprint }
+  )
+  ∧
+  Opt.compile (.or x₁ x₂) εnv = (do
+    let term ← SymCC.compile (.or x₁ x₂) εnv
+    let footprint := footprint (.or x₁ x₂) εnv
+    .ok { term, footprint }
+  )
+:= by
+  constructor
+  all_goals {
+    simp [Opt.compile, SymCC.compile, footprint]
+    rw [Opt.compile.correctness x₁ εnv, Opt.compile.correctness x₂ εnv]
+    simp [Opt.compileAnd, SymCC.compileAnd, Opt.compileOr, SymCC.compileOr, footprint.ofBranch, EmptyCollection.emptyCollection]
+    cases h₁ : SymCC.compile x₁ εnv <;> simp only [Except.bind_ok, Except.bind_err]
+    case ok t₁ =>
+      cases h₂ : SymCC.compile x₂ εnv <;> simp only [Except.bind_ok, Except.bind_err]
+      case error e => split <;> simp [*]
+      case ok t₂ =>
+        split <;> simp [*]
+        split <;> simp at *
+        split <;> simp [*]
+        first
+        | rw [Data.Set.union_empty_right (Data.Set.union_wf _ _)]
+        | rw [Data.Set.union_empty_right (footprint_wf _ _)]
+  }
+termination_by 1 + 2 * sizeOf x₁ + 2 * sizeOf x₂
+
+/--
+Correctness theorem for `Opt.compile` -- `unaryApp` case
+-/
+theorem Opt.compile.correctness.unaryApp (op : UnaryOp) (x : Expr) (εnv : SymEnv) :
+  Opt.compile (.unaryApp op x) εnv = (do
+    let term ← SymCC.compile (.unaryApp op x) εnv
+    let footprint := footprint (.unaryApp op x) εnv
+    .ok { term, footprint }
+  )
+:= by
+  simp [Opt.compile, SymCC.compile, footprint]
+  rw [Opt.compile.correctness x εnv]
+  cases h₁ : SymCC.compile x εnv <;> simp
+  rw [Opt.compileApp₁.correctness op]
+  simp [Opt.CompileResult.mapTerm]
+termination_by 1 + 2 * sizeOf x
+
+/--
+Correctness theorem for `Opt.compile` -- `binaryApp` case
+-/
+theorem Opt.compile.correctness.binaryApp (op : BinaryOp) (x₁ x₂ : Expr) (εnv : SymEnv) :
+  Opt.compile (.binaryApp op x₁ x₂) εnv = (do
+    let term ← SymCC.compile (.binaryApp op x₁ x₂) εnv
+    let footprint := footprint (.binaryApp op x₁ x₂) εnv
+    .ok { term, footprint }
+  )
+:= by
+  simp [Opt.compile, SymCC.compile, footprint]
+  rw [Opt.compile.correctness x₁ εnv, Opt.compile.correctness x₂ εnv]
+  cases h₁ : SymCC.compile x₁ εnv <;> simp
+  case ok t₁ =>
+    cases h₂ : SymCC.compile x₂ εnv <;> simp
+    case ok t₂ =>
+      rw [Opt.compileApp₂.correctness op]
+      simp [Opt.CompileResult.mapTerm]
+      cases h : SymCC.compileApp₂ op (Factory.option.get t₁) (Factory.option.get t₂) εnv.entities <;> simp
+      case ok t =>
+        rw [Opt.directFootprint.correctness (t := Factory.ifSome t₁ (Factory.ifSome t₂ t)) (εnv := εnv) (x := .binaryApp op x₁ x₂)]
+        · conv => rhs ; rw [Data.Set.union_assoc, Data.Set.union_comm]
+        · -- here we have to show that the `t` and `x` arguments we chose for `Opt.directFootprint.correctness` in the `rw` above correspond to each other correctly
+          simp [SymCC.compile, h₁, h₂, h]
+termination_by 1 + 2 * sizeOf x₁ + 2 * sizeOf x₂
+decreasing_by all_goals {
+  have : ∀ x : Expr, sizeOf x > 0 := by
+    intro x ; cases x <;> simp [sizeOf, Expr._sizeOf_1] <;> omega
+  have hx₁ := this x₁
+  have hx₂ := this x₂
+  omega
+}
+
+/--
+Correctness theorem for `Opt.compile` -- `getAttr` case
+-/
+theorem Opt.compile.correctness.getAttr (expr : Expr) (attr : Attr) (εnv : SymEnv) :
+  Opt.compile (.getAttr expr attr) εnv = (do
+    let term ← SymCC.compile (.getAttr expr attr) εnv
+    let footprint := footprint (.getAttr expr attr) εnv
+    .ok { term, footprint }
+  )
+:= by
+  simp [Opt.compile, SymCC.compile, footprint]
+  rw [Opt.compile.correctness expr εnv]
+  cases h₁ : SymCC.compile expr εnv <;> simp
+  case ok t =>
+    rw [Opt.compileGetAttr.correctness]
+    simp only [Opt.CompileResult.mapTerm, bind_assoc, Except.bind_ok]
+    simp_do_let compileGetAttr (Factory.option.get t) attr εnv.entities ; rename_i t' h₂
+    simp only [Except.ok.injEq, Opt.CompileResult.mk.injEq, true_and]
+    rw [Opt.directFootprint.correctness (t := Factory.ifSome t t') (x := .getAttr expr attr) (εnv := εnv)]
+    · apply Data.Set.union_comm
+    · -- here we have to show that the `t` and `x` arguments we chose for `Opt.directFootprint.correctness` in the `rw` above correspond to each other correctly
+      simp [SymCC.compile, h₁, h₂]
+termination_by 1 + 2 * sizeOf expr
+
+/--
+Correctness theorem for `Opt.compile` -- `hasAttr` case
+-/
+theorem Opt.compile.correctness.hasAttr (expr : Expr) (attr : Attr) (εnv : SymEnv) :
+  Opt.compile (.hasAttr expr attr) εnv = (do
+    let term ← SymCC.compile (.hasAttr expr attr) εnv
+    let footprint := footprint (.hasAttr expr attr) εnv
+    .ok { term, footprint }
+  )
+:= by
+  simp [Opt.compile, SymCC.compile, footprint]
+  rw [Opt.compile.correctness expr εnv]
+  cases h₁ : SymCC.compile expr εnv <;> simp
+  case ok t =>
+    rw [Opt.compileHasAttr.correctness]
+    simp only [Opt.CompileResult.mapTerm, bind_assoc, Except.bind_ok]
+termination_by 1 + 2 * sizeOf expr
+
+/--
+Correctness theorem for `Opt.compile` -- `set` case
+-/
+theorem Opt.compile.correctness.set (ls : List Expr) (εnv : SymEnv) :
+  Opt.compile (.set ls) εnv = (do
+    let term ← SymCC.compile (.set ls) εnv
+    let footprint := footprint (.set ls) εnv
+    .ok { term, footprint }
+  )
+:= by
+  simp [Opt.compile, SymCC.compile, footprint]
+  rw [List.mapM₁_eq_mapM (Opt.compile · εnv), List.mapM₁_eq_mapM (SymCC.compile · εnv)]
+  rw [List.mapUnion_attach (footprint · εnv)]
+  simp_do_let ls.mapM (Opt.compile · εnv) <;> rename_i hmap₁
+  <;> simp_do_let ls.mapM (SymCC.compile · εnv) <;> rename_i hmap₂
+  case error.error e₁ e₂ =>
+    simp only [Except.error.injEq]
+    apply both_lists_error_then_errors_same hmap₁ hmap₂
+    intro x hx
+    have := List.sizeOf_lt_of_mem hx -- for termination
+    exact Opt.compile.correctness x εnv
+  case ok.error ts e =>
+    exfalso
+    replace ⟨x, hx, hmap₂⟩ := List.mapM_error_implies_exists_error hmap₂
+    replace ⟨t, ht, hmap₁⟩ := List.mapM_ok_implies_all_ok hmap₁ x hx
+    have := List.sizeOf_lt_of_mem hx -- for termination
+    rw [Opt.compile.correctness] at hmap₁
+    simp [hmap₂] at hmap₁
+  case error.ok e ts =>
+    exfalso
+    replace ⟨x, hx, hmap₁⟩ := List.mapM_error_implies_exists_error hmap₁
+    replace ⟨t, ht, hmap₂⟩ := List.mapM_ok_implies_all_ok hmap₂ x hx
+    have := List.sizeOf_lt_of_mem hx -- for termination
+    rw [Opt.compile.correctness] at hmap₁
+    simp [hmap₂] at hmap₁
+  case ok.ok ts₁ ts₂ =>
+    rw [Opt.compileSet.correctness]
+    suffices
+      SymCC.compileSet (List.map Opt.CompileResult.term ts₁) = SymCC.compileSet ts₂
+      ∧ ts₁.mapUnion Opt.CompileResult.footprint = ls.mapUnion (footprint · εnv)
+      by simp [this]
+    have ⟨h₁, h₂⟩ := both_lists_ok_then_elts_correspond hmap₁ hmap₂ (by
+      intro x hx
+      have := List.sizeOf_lt_of_mem hx -- for termination
+      exact Opt.compile.correctness x εnv
+    )
+    subst ts₂ ; simp
+    apply Data.Set.map_eqv_implies_mapUnion_eq (by simp [h₂, List.Equiv.refl])
+termination_by 1 + 2 * sizeOf ls
+
+/--
+Correctness theorem for `Opt.compile` -- `record` case
+-/
+theorem Opt.compile.correctness.record (m : List (Attr × Expr)) (εnv : SymEnv) :
+  Opt.compile (.record m) εnv = (do
+    let term ← SymCC.compile (.record m) εnv
+    let footprint := footprint (.record m) εnv
+    .ok { term, footprint }
+  )
+:= by
+  simp [Opt.compile, SymCC.compile, footprint]
+  simp only [List.mapM₂_eq_mapM (λ x => do Except.ok (x.fst, ← Opt.compile x.snd εnv)) m]
+  simp only [List.mapM₂_eq_mapM (λ x => do Except.ok (x.fst, ← SymCC.compile x.snd εnv)) m]
+  rw [List.mapUnion_attach₂ (λ x => footprint x.snd εnv)]
+  simp_do_let m.mapM (m := SymCC.Result) _ <;> rename_i hmap₁
+  <;> simp_do_let m.mapM (m := SymCC.Result) _ <;> rename_i hmap₂
+  case error.error e₁ e₂ =>
+    simp only [Except.error.injEq]
+    apply both_lists_pairs_error_then_errors_same hmap₁ hmap₂
+    intro pair hpair
+    have := List.sizeOf_lt_of_mem hpair -- for termination
+    have : sizeOf pair.snd < sizeOf pair := by simp [sizeOf, Prod._sizeOf_1] ; omega
+    exact Opt.compile.correctness pair.snd εnv
+  case ok.error ts e =>
+    exfalso
+    replace ⟨x, hx, hmap₂⟩ := List.mapM_error_implies_exists_error hmap₂
+    replace ⟨t, ht, hmap₁⟩ := List.mapM_ok_implies_all_ok hmap₁ x hx
+    have := List.sizeOf_lt_of_mem hx -- for termination
+    have : sizeOf x.snd < sizeOf x := by simp [sizeOf, Prod._sizeOf_1] ; omega
+    rw [Opt.compile.correctness] at hmap₁
+    simp [do_error] at hmap₂
+    simp [hmap₂] at hmap₁
+  case error.ok e ts =>
+    exfalso
+    replace ⟨x, hx, hmap₁⟩ := List.mapM_error_implies_exists_error hmap₁
+    replace ⟨t, ht, hmap₂⟩ := List.mapM_ok_implies_all_ok hmap₂ x hx
+    have := List.sizeOf_lt_of_mem hx -- for termination
+    have : sizeOf x.snd < sizeOf x := by simp [sizeOf, Prod._sizeOf_1] ; omega
+    rw [Opt.compile.correctness] at hmap₁
+    simp [do_error] at hmap₁
+    simp [hmap₁] at hmap₂
+  case ok.ok ts₁ ts₂ =>
+    rw [Opt.compileRecord.correctness]
+    simp only [Except.ok.injEq, Opt.CompileResult.mk.injEq]
+    have ⟨h₁, h₂⟩ := both_lists_pairs_ok_then_elts_correspond hmap₁ hmap₂ (by
+      intro pair hpair
+      have := List.sizeOf_lt_of_mem hpair -- for termination
+      have : sizeOf pair.snd < sizeOf pair := by simp [sizeOf, Prod._sizeOf_1] ; omega
+      exact Opt.compile.correctness pair.snd εnv
+    )
+    subst ts₂ ; simp
+    apply Data.Set.map_eqv_implies_mapUnion_eq (by simp [h₂, List.Equiv.refl])
+termination_by 1 + 2 * sizeOf m
+
+/--
+Correctness theorem for `Opt.compile` -- `call` case
+-/
+theorem Opt.compile.correctness.call (xfn : ExtFun) (args : List Expr) (εnv : SymEnv) :
+  Opt.compile (.call xfn args) εnv = (do
+    let term ← SymCC.compile (.call xfn args) εnv
+    let footprint := footprint (.call xfn args) εnv
+    .ok { term, footprint }
+  )
+:= by
+  simp [Opt.compile, SymCC.compile, footprint]
+  rw [List.mapM₁_eq_mapM (Opt.compile · εnv), List.mapM₁_eq_mapM (SymCC.compile · εnv)]
+  rw [List.mapUnion_attach (footprint · εnv)]
+  simp_do_let args.mapM (Opt.compile · εnv) <;> rename_i hmap₁
+  <;> simp_do_let args.mapM (SymCC.compile · εnv) <;> rename_i hmap₂
+  case error.error e₁ e₂ =>
+    simp only [Except.error.injEq]
+    apply both_lists_error_then_errors_same hmap₁ hmap₂
+    intro x hx
+    have := List.sizeOf_lt_of_mem hx -- for termination
+    exact Opt.compile.correctness x εnv
+  case ok.error ts e =>
+    exfalso
+    replace ⟨x, hx, hmap₂⟩ := List.mapM_error_implies_exists_error hmap₂
+    replace ⟨t, ht, hmap₁⟩ := List.mapM_ok_implies_all_ok hmap₁ x hx
+    have := List.sizeOf_lt_of_mem hx -- for termination
+    rw [Opt.compile.correctness] at hmap₁
+    simp [hmap₂] at hmap₁
+  case error.ok e ts =>
+    exfalso
+    replace ⟨x, hx, hmap₁⟩ := List.mapM_error_implies_exists_error hmap₁
+    replace ⟨t, ht, hmap₂⟩ := List.mapM_ok_implies_all_ok hmap₂ x hx
+    have hterm := List.sizeOf_lt_of_mem hx -- for termination
+    rw [Opt.compile.correctness] at hmap₁
+    simp [hmap₂] at hmap₁
+  case ok.ok ts₁ ts₂ =>
+    rw [Opt.compileCall.correctness]
+    · suffices
+        SymCC.compileCall xfn (List.map Opt.CompileResult.term ts₁) = SymCC.compileCall xfn ts₂
+        ∧ ts₁.mapUnion Opt.CompileResult.footprint = args.mapUnion (footprint · εnv)
+        by simp [this]
+      have ⟨h₁, h₂⟩ := both_lists_ok_then_elts_correspond hmap₁ hmap₂ (by
+        intro x hx
+        have := List.sizeOf_lt_of_mem hx -- for termination
+        exact Opt.compile.correctness x εnv
+      )
+      subst ts₂ ; simp
+      apply Data.Set.map_eqv_implies_mapUnion_eq (by simp [h₂, List.Equiv.refl])
+    case hwf =>
+      intro res hres
+      have ⟨arg, harg, h₁⟩ := List.mapM_ok_implies_all_from_ok hmap₁ res hres
+      exact Opt.compile_footprint_wf h₁
+termination_by 1 + 2 * sizeOf args
+
+/--
+Correctness theorem for `Opt.compile`:
+
+`Opt.compile` produces the same `term` as `SymCC.compile`, and
+`Opt.compile` produces the same `footprint` as `footprint`
+-/
+theorem Opt.compile.correctness (x : Expr) (εnv : SymEnv) :
+  Opt.compile x εnv = (do
+    let term ← SymCC.compile x εnv
+    let footprint := footprint x εnv
+    .ok { term, footprint }
+  )
+:= by
+  cases x
+  case lit p => exact Opt.compile.correctness.lit p εnv
+  case var v => exact Opt.compile.correctness.var v εnv
+  case and x₁ x₂ | or x₁ x₂ =>
+    first
+    | exact (Opt.compile.correctness.andor x₁ x₂ εnv).left
+    | exact (Opt.compile.correctness.andor x₁ x₂ εnv).right
+  case ite x₁ x₂ x₃       => exact Opt.compile.correctness.ite x₁ x₂ x₃ εnv
+  case unaryApp op x₁     => exact Opt.compile.correctness.unaryApp op x₁ εnv
+  case binaryApp op x₁ x₂ => exact Opt.compile.correctness.binaryApp op x₁ x₂ εnv
+  case getAttr x₁ attr    => exact Opt.compile.correctness.getAttr x₁ attr εnv
+  case hasAttr x₁ attr    => exact Opt.compile.correctness.hasAttr x₁ attr εnv
+  case set xs             => exact Opt.compile.correctness.set xs εnv
+  case record m           => exact Opt.compile.correctness.record m εnv
+  case call xfn args      => exact Opt.compile.correctness.call xfn args εnv
+termination_by 2 * sizeOf x
+
+end
